src/TV/eq_tv_dec.v
@@ -1,7 +1,7 @@
 Add LoadPath "../ssa/ott".
 Add LoadPath "../ssa/monads".
 Add LoadPath "../ssa".
-(*Add LoadPath "../../../theory/metatheory".*)
+Add LoadPath "../../../theory/metatheory_8.3".
 Require Import ssa_def.
 Require Import ssa_lib.
 Require Import List.
