src/TV/sub_tv.v
@@ -1,0 +1,124 @@
+Add LoadPath "../ssa/ott".
+Add LoadPath "../ssa/monads".
+Add LoadPath "../ssa".
+Add LoadPath "../ssa/compcert".
+Add LoadPath "../../../theory/metatheory_8.3".
+Require Import ssa_def.
+Require Import ssa_lib.
+Require Import List.
+Require Import targetdata.
+Require Import monad.
+Require Import Arith.
+Require Import Metatheory.
+Require Import ssa_mem.
+Require Import genericvalues.
+Require Import ssa_dynamic.
+Require Import opsem_pp.
+Require Import trace.
+Require Import symexe_def.
+Require Import symexe_lib.
+Require Import symexe_complete.
+Require Import symexe_sound.
+Require Import seop_llvmop.
+Require Import assoclist.
+Require Import ssa_props.
+Require Import sub_tv_dec.
+Require Import Coq.Bool.Sumbool.
+
+Export SimpleSE.
+
+Definition tv_cmds (nbs1 nbs2 : list nbranch) :=
+sumbool2bool _ _ (sstate_sub_dec (se_cmds sstate_init nbs1) (se_cmds sstate_init nbs2)
+                    (se_cmds_init_uniq nbs1)).
+
+Definition tv_subblock (sb1 sb2:subblock) :=
+match (sb1, sb2) with
+| (mkSB nbs1 call1 iscall1, mkSB nbs2 call2 iscall2) =>
+  let st1 := se_cmds sstate_init nbs1 in
+  let st2 := se_cmds sstate_init nbs2 in
+  let cl1 := se_call st1 call1 iscall1 in
+  let cl2 := se_call st2 call2 iscall2 in
+   (sumbool2bool _ _ (sstate_sub_dec st1 st2 (se_cmds_init_uniq nbs1))) &&
+   (sumbool2bool _ _ (cmd_dec call1 call2))
+end.
+
+Fixpoint tv_subblocks (sbs1 sbs2:list subblock) :=
+match (sbs1, sbs2) with
+| (nil, nil) => true
+| (sb1::sbs1', sb2::sbs2') => 
+   (tv_subblock sb1 sb2) && (tv_subblocks sbs1' sbs2')
+| _ => false
+end.
+
+Fixpoint tv_phinodes (ps1 ps2:phinodes) :=
+match (ps1, ps2) with
+| (nil, nil) => true
+| (p1::ps1', p2::ps2') => 
+    sumbool2bool _ _ (phinode_dec p1 p2) && tv_phinodes ps1' ps2'
+| _ => false
+end.
+
+Definition tv_block (b1 b2:block) :=
+match (b1, b2) with
+| (block_intro l1 ps1 cs1 tmn1, block_intro l2 ps2 cs2 tmn2) =>
+  match (cmds2sbs cs1, cmds2sbs cs2) with
+  | ((sbs1, nbs1), (sbs2, nbs2)) =>
+    sumbool2bool _ _ (eq_atom_dec l1 l2) &&
+    tv_phinodes ps1 ps2 &&
+    tv_subblocks sbs1 sbs2 &&
+    tv_cmds nbs1 nbs2 &&
+    sumbool2bool _ _ (terminator_dec tmn1 tmn2)
+  end
+end.
+
+Fixpoint tv_blocks (bs1 bs2:blocks):=
+match (bs1, bs2) with
+| (nil, nil) => true
+| (b1::bs1', b2::bs2') => tv_block b1 b2 && tv_blocks bs1' bs2'
+| _ => false
+end.
+
+Definition tv_fdef (f1 f2:fdef) :=
+match (f1, f2) with
+| (fdef_intro fh1 lb1, fdef_intro fh2 lb2) =>
+  sumbool2bool _ _ (fheader_dec fh1 fh2) &&
+  tv_blocks lb1 lb2
+end.
+
+Fixpoint tv_products (Ps1 Ps2:products):=
+match (Ps1, Ps2) with
+| (nil, nil) => true
+| (product_fdec f1::Ps1', product_fdec f2::Ps2') => 
+  sumbool2bool _ _ (fdec_dec f1 f2) &&
+  tv_products Ps1' Ps2'
+| (product_fdef f1::Ps1', product_fdef f2::Ps2') => 
+  tv_fdef f1 f2 && tv_products Ps1' Ps2'
+| (product_gvar gvar1::Ps1', product_gvar gvar2::Ps2') => 
+  sumbool2bool _ _ (gvar_dec gvar1 gvar2) &&
+  tv_products Ps1' Ps2'
+| _ => false
+end.
+
+Definition tv_module (m1 m2:module) :=
+match (m1, m2) with
+| (module_intro los1 nts1 Ps1, module_intro los2 nts2 Ps2) =>
+  sumbool2bool _ _ (layouts_dec los1 los2) &&
+  sumbool2bool _ _ (namedts_dec nts1 nts2) &&
+  tv_products Ps1 Ps2
+end.
+
+Fixpoint tv_system (S1 S2:system) :=
+match (S1, S2) with
+| (nil, nil) => true
+| (m1::S1', m2::S2') => tv_module m1 m2 && tv_system S1' S2'
+| _ => false
+end.
+
+Ltac sumbool_simpl :=
+  repeat
+  match goal with
+  | [ H:sumbool2bool _ _ _ = true |- _ ] => apply sumbool2bool_true in H
+  | [ H:is_true(sumbool2bool _ _ _) |- _ ] => apply sumbool2bool_true in H
+  | [ H:tv_cmds _ _ = true |- _ ] => unfold is_true in H; apply sumbool2bool_true in H
+  | [ H:is_true(tv_cmds _ _) |- _ ] => unfold is_true in H; apply sumbool2bool_true in H
+  end.
