src/TV/sub_tv_dec.v
@@ -1,0 +1,84 @@
+(* Start CoqIDE at ./src/TV *)
+Add LoadPath "../ssa/ott".
+Add LoadPath "../ssa/monads".
+Add LoadPath "../ssa/compcert".
+Add LoadPath "../ssa".
+Add LoadPath "../../../theory/metatheory_8.3".
+Require Import ssa_def.
+Require Import ssa_lib.
+Require Import List.
+Require Import targetdata.
+Require Import monad.
+Require Import Arith.
+Require Import Metatheory.
+Require Import ssa_mem.
+Require Import genericvalues.
+Require Import ssa_dynamic.
+Require Import trace.
+Require Import assoclist.
+Require Import ssa_props.
+Require Import CoqListFacts.
+Require Import symexe_def.
+Require Import symexe_lib.
+Require Import eq_tv_dec.
+
+Export SimpleSE.
+
+Definition sub_sstate s1 s2 := 
+  s1.(STerms) <<<= s2.(STerms) /\ s1.(SMem) = s2.(SMem) /\
+  s1.(SFrame) = s2.(SFrame) /\ s1.(SEffects) = s2.(SEffects).
+
+Notation "s1 <<= s2" := (sub_sstate s1 s2) (at level 70, no associativity).
+
+Lemma smap_sub_dec : forall (sm1 sm2:smap), uniq sm1 -> {sm1 <<<= sm2}+{~sm1 <<<= sm2}.
+Proof.
+  induction sm1.  
+    intros. left. intros i i_in_nil. fsetdec. 
+
+    intros sm2 Huniq. 
+    destruct a as [id st1].
+    remember (lookupAL _ sm2 id) as Lookup.
+    destruct Lookup as [st2 | _].
+      destruct (@sterm_dec st1 st2); subst.
+        destruct_uniq.
+        destruct (@IHsm1 sm2 Huniq) as [sm1_sub_sm2 | sm1_nsub_sm2].
+          left. simpl_env.
+          apply subAL_app1; auto.
+            intros i Hi_in_dom. simpl in *.
+            destruct (@eq_dec atom (EqDec_eq_of_EqDec atom EqDec_atom) i id); subst.
+              rewrite <- HeqLookup; auto.
+              fsetdec.
+
+          right. simpl_env.
+          apply subAL_app2; auto.
+            intros id0 Hid0_in.
+            assert (id0=id) as Eq. simpl in Hid0_in. fsetdec.
+            subst.
+            simpl. 
+            destruct (@eq_dec atom (EqDec_eq_of_EqDec atom EqDec_atom) id id); auto.
+              contradict n; auto.
+        right. intro J. assert (H:=@J id). simpl in H.
+        destruct (@eq_dec atom (EqDec_eq_of_EqDec atom EqDec_atom) id id); auto.
+          rewrite <- HeqLookup in H. injection H; auto.
+      right. intro J. assert (H:=@J id). simpl in H.
+      destruct (@eq_dec atom (EqDec_eq_of_EqDec atom EqDec_atom) id id); auto.
+        rewrite <- HeqLookup in H.
+        assert (ret st1 = merror) as F. auto.
+        inversion F.
+Qed.
+
+Lemma sstate_sub_dec : forall (sts1 sts2:sstate), 
+  uniq sts1.(STerms) -> {sts1<<=sts2} + {~sts1<<=sts2}.
+Proof.
+Ltac done_right := 
+  right; intro J ; destruct J as [ J1 [J2 [J3 J4]]]; simpl in *; auto.
+
+  intros sts1 sts2 Huniq.
+  destruct sts1 as [st1 sm1 sf1 se1].
+  destruct sts2 as [st2 sm2 sf2 se2].
+  destruct (@sterms_dec se1 se2); subst; try solve [auto | done_right].
+  destruct (@sframe_dec sf1 sf2); subst; try solve [auto | done_right].
+  destruct (@smem_dec sm1 sm2); subst; try solve [auto | done_right].
+  destruct (@smap_sub_dec st1 st2 Huniq); subst; try solve [left; split; auto | done_right].
+Qed.
+
