src/TV/symexe_lib.v
@@ -1,0 +1,2698 @@
+Add LoadPath "../ssa/ott".
+Add LoadPath "../ssa/monads".
+Add LoadPath "../ssa/compcert".
+Add LoadPath "../ssa".
+Add LoadPath "../../../theory/metatheory_8.3".
+Require Import ssa_def.
+Require Import ssa_lib.
+Require Import List.
+Require Import targetdata.
+Require Import monad.
+Require Import Arith.
+Require Import Metatheory.
+Require Import ssa_mem.
+Require Import genericvalues.
+Require Import ssa_dynamic.
+Require Import opsem_pp.
+Require Import trace.
+Require Import assoclist.
+Require Import ssa_props.
+Require Import CoqListFacts.
+Require Import Coqlib.
+Require Import symexe_def.
+
+Export SimpleSE.
+
+(* cmd2sbs *)
+
+Lemma cmds2sbs_nil_inv : forall cs,
+  cmds2sbs cs = (nil, nil) ->
+  cs = nil.
+Proof.
+  destruct cs; intros; auto.
+    simpl in H.
+    destruct (isCallInst_dec c).
+      destruct (cmds2sbs cs).
+      destruct l0.
+        inversion H.
+        destruct s. inversion H.
+      destruct (cmds2sbs cs).
+      inversion H.
+Qed.
+
+Lemma cmds2sb_inv : forall cs sb,
+  cmds2sbs cs = (sb::nil, nil) ->
+  exists cs', exists call0,
+    cs = cs'++call0::nil /\
+    cmds2sbs cs' = (nil, NBs sb) /\
+    call_cmd sb = call0.
+Proof.
+  induction cs; intros; simpl in *.
+    inversion H.
+
+    remember (cmds2sbs cs) as R.
+    remember (isCallInst_dec a) as R'.
+    destruct R'.
+      destruct R.
+      destruct l0.
+        inversion H.
+
+        destruct s. inversion H; subst. clear H.
+        destruct (@IHcs (mkSB NBs0 call_cmd0 call_cmd_isCall0)) as [cs' [call0 [J1 [J2 J3]]]]; subst; auto.
+        clear IHcs.
+        simpl in *.
+        exists (a::cs').
+        exists (call_cmd0).
+        split; auto.
+        split; auto.
+          simpl.
+          rewrite J2.
+          rewrite <- HeqR'. auto.
+
+      destruct R.
+      inversion H; subst. clear H.
+      symmetry in HeqR.
+      apply cmds2sbs_nil_inv in HeqR. subst.
+      exists nil. exists a.
+      split; auto.
+Qed.
+
+Definition dbCmds__cmds2nbs : forall TD lc als gl Mem1 cs lc' als' Mem2 tr, 
+  dbCmds TD gl lc als Mem1 cs lc' als' Mem2 tr ->
+  exists nbs, cmds2sbs cs = (nil, nbs).
+Proof.
+  intros.
+  induction H; simpl.
+    exists nil. auto.
+
+    destruct IHdbCmds as [nbs J].
+    destruct (isCallInst_dec c).
+      rewrite J. exists (mkNB c e::nbs). auto.
+
+      apply dbCmd_isNotCallInst in H.
+      rewrite e in H. inversion H.
+Qed.
+
+Lemma dbCall_isCallInst : forall S TD Ps lc gl fs Mem1 c lc' Mem2 tr,
+  dbCall S TD Ps fs gl lc Mem1 c lc' Mem2 tr ->
+  Instruction.isCallInst c = true.
+Proof.
+  intros S TD Ps lc gl fs Mem1 c lc' Mem2 tr HdbCall.
+  induction HdbCall; auto.
+Qed.
+
+Lemma cmdscall2sbs : forall cs call0 nbs
+  (isCall0:Instruction.isCallInst call0=true),
+  cmds2sbs cs = (nil, nbs) ->
+  isCallInst_dec call0 = right isCall0 ->
+  cmds2sbs (cs++call0::nil) = (mkSB nbs call0 isCall0::nil, nil).
+Proof.
+  induction cs; intros; simpl in *.
+    inversion H; subst.
+    rewrite H0. auto.
+
+    destruct (isCallInst_dec a).
+      remember (cmds2sbs cs) as R.
+      destruct R.
+      destruct l0.
+        inversion H; subst. clear H.
+        apply IHcs with (nbs:=l1) in H0; auto.
+        rewrite H0; auto.
+     
+        destruct s. inversion H.
+
+      destruct (cmds2sbs cs).
+      inversion H.
+Qed.
+
+Lemma dbSubblock__cmds2sb : forall S TD Ps fs gl lc1 als1 Mem1 cs lc2 als2 Mem2 tr,
+  dbSubblock S TD Ps fs gl lc1 als1 Mem1 cs lc2 als2 Mem2 tr ->
+  exists sb, cmds2sbs cs = (sb::nil, nil).
+Proof.
+  intros.
+  inversion H; subst.
+  apply dbCmds__cmds2nbs in H0.
+  destruct H0 as [nbs H0].
+  remember (isCallInst_dec call0) as R.
+  destruct R.
+    apply dbCall_isCallInst in H1.
+    rewrite e in H1. inversion H1.
+
+    exists (mkSB nbs call0 e).
+    apply cmdscall2sbs; auto.
+Qed.
+
+Lemma cmds_cons2sbs : forall cs cs' sb sbs',
+  cmds2sbs cs = (sb::nil, nil) ->
+  cmds2sbs cs' = (sbs', nil) ->
+  cmds2sbs (cs++cs') = (sb::sbs', nil).
+Proof.
+  induction cs; intros; simpl.
+    simpl in H. inversion H.
+
+    simpl in H.
+    destruct (isCallInst_dec a).
+      remember (cmds2sbs cs) as R.
+      destruct R.
+        destruct l0.
+          inversion H.
+
+          destruct s. inversion H; subst. clear H.
+          apply IHcs with (sb:=mkSB NBs0 call_cmd0 call_cmd_isCall0) in H0; auto.
+          clear IHcs.
+          rewrite H0. auto.
+ 
+      remember (cmds2sbs cs) as R.
+      destruct R.
+      inversion H; subst. clear H.
+      symmetry in HeqR.
+      apply cmds2sbs_nil_inv in HeqR. subst.
+      simpl.
+      rewrite H0. auto.
+Qed.
+
+Lemma dbSubblocks__cmds2sbs : forall S TD Ps fs gl lc1 als1 Mem1 cs lc2 als2 Mem2 tr,
+  dbSubblocks S TD Ps fs gl lc1 als1 Mem1 cs lc2 als2 Mem2 tr ->
+  exists sbs, cmds2sbs cs = (sbs, nil).
+Proof.
+  intros.
+  induction H; simpl.
+    exists nil. auto.
+
+    apply dbSubblock__cmds2sb in H.
+    destruct H as [sb H].
+    destruct IHdbSubblocks as [sbs H1].
+    exists (sb::sbs).
+    apply cmds_cons2sbs; auto.
+Qed.
+
+Lemma cmds_cons2sbs_inv : forall cs cs' sbs0 sb sbs',
+  cmds2sbs (cs++cs') = (sbs0, nil) ->
+  cmds2sbs cs = (sb::nil, nil) ->
+  cmds2sbs cs' = (sbs', nil) ->
+  sbs0 = sb::sbs'.
+Proof.
+  intros.
+  apply cmds_cons2sbs with (cs':=cs')(sbs':=sbs') in H0; auto.
+  rewrite H in H0.
+  inversion H0; auto.
+Qed.
+
+Lemma cmds2sbs_cons_inv : forall cs0 sb sbs',
+  cmds2sbs cs0 = (sb::sbs', nil) ->
+  exists cs, exists cs',
+    cmds2sbs cs = (sb::nil, nil) /\
+    cmds2sbs cs' = (sbs', nil) /\
+    cs0 = cs++cs'.
+Proof.
+  induction cs0; intros.
+    simpl in H. inversion H.
+
+    simpl in H.
+    remember (isCallInst_dec a) as R.
+    remember (cmds2sbs cs0) as R'.
+    destruct R.
+      destruct R'.
+        destruct l0.
+          inversion H.
+
+          destruct s. inversion H; subst. clear H.
+          destruct (@IHcs0 (mkSB NBs0 call_cmd0 call_cmd_isCall0) sbs') as [cs [cs' [J1 [J2 J3]]]]; subst; auto.
+          exists (a::cs). exists cs'.
+          split; auto.
+            simpl.
+            rewrite <- HeqR.
+            rewrite J1. auto.
+
+      destruct R'.
+      inversion H; subst. clear H.
+      destruct sbs'.
+        symmetry in HeqR'.
+        apply cmds2sbs_nil_inv in HeqR'. subst.
+        exists (a::nil). exists nil.
+        simpl. rewrite <- HeqR. auto.
+
+        destruct (@IHcs0 s sbs') as [cs [cs' [J1 [J2 J3]]]]; subst; auto.
+        exists (a::nil). exists (cs++cs').
+        simpl. rewrite <- HeqR. auto.
+Qed.
+
+Lemma cmds_rcons2sbs : forall cs cs' sbs nbs,
+  cmds2sbs cs = (sbs, nil) ->
+  cmds2sbs cs' = (nil, nbs) ->
+  cmds2sbs (cs++cs') = (sbs, nbs).
+Proof.
+  induction cs; intros.
+    simpl in H. inversion H; subst. auto.
+
+    simpl in *.
+    remember (cmds2sbs cs) as R.
+    destruct (isCallInst_dec a).
+      destruct R.
+        destruct l0.
+          inversion H.
+
+          destruct s. inversion H; subst. clear H.
+          apply IHcs with (sbs:=mkSB NBs0 call_cmd0 call_cmd_isCall0::l0) in H0; auto.
+          rewrite H0. auto.
+
+      destruct R.
+      inversion H; subst. clear H.
+      apply IHcs with (sbs:=l0) in H0; auto.
+      rewrite H0. auto.
+Qed.
+
+Lemma cmds_rcons2sbs_inv : forall cs cs' sbs0 nbs0 sbs nbs,
+  cmds2sbs (cs++cs') = (sbs0, nbs0) ->
+  cmds2sbs cs = (sbs, nil) ->
+  cmds2sbs cs' = (nil, nbs) ->
+  sbs0 = sbs /\ nbs0 = nbs.
+Proof.
+  intros.
+  apply cmds_rcons2sbs with (cs':=cs')(nbs:=nbs) in H0; auto.
+  rewrite H in H0. inversion H0; auto.
+Qed.
+ 
+Lemma cmds2nbranchs__cmds2nbs : forall cs nbs,
+  cmds2nbranchs cs = Some nbs ->
+  cmds2sbs cs = (nil, nbs).
+Proof.
+  induction cs; intros.
+    simpl in H. inversion H; auto.
+
+    simpl in *.
+    unfold cmd2nbranch in H.
+    destruct (isCallInst_dec a).
+      destruct (cmds2sbs cs).
+        remember (cmds2nbranchs cs) as R.
+        destruct R.
+          inversion H; subst. clear H.
+          assert (ret l2 = ret l2) as EQ. auto.
+          apply IHcs in EQ.
+          inversion EQ; subst. auto.
+
+          inversion H.
+      inversion H.
+Qed.
+
+Lemma cmds2nbs__nbranchs2cmds : forall nbs cs,
+  cmds2sbs cs = (nil, nbs) ->
+  nbranchs2cmds nbs = cs.
+Proof.
+  induction nbs; intros.
+    apply cmds2sbs_nil_inv in H. subst. auto.
+
+    simpl.
+    destruct a.
+    destruct cs.
+      simpl in H. inversion H.
+
+      simpl in H.
+      destruct (isCallInst_dec c).
+        remember (cmds2sbs cs) as R.
+        destruct R.
+        destruct l0.
+          inversion H; subst.
+          rewrite IHnbs with (cs:=cs); auto.
+
+          destruct s.
+          inversion H; subst.
+
+        destruct (cmds2sbs cs).
+        inversion H.
+Qed.
+
+
+Lemma cmds2nbranchs__nbranchs2cmds : forall cs nbs,
+  cmds2nbranchs cs = Some nbs ->
+  nbranchs2cmds nbs = cs.
+Proof.
+  intros.
+  apply cmds2nbs__nbranchs2cmds.
+  apply cmds2nbranchs__cmds2nbs; auto.
+Qed.
+
+Lemma cmds2sbs_inv : forall cs sbs nbs,
+  cmds2sbs cs = (sbs, nbs) ->
+  exists cs1, exists cs2, 
+    cs = cs1++cs2 /\
+    cmds2sbs cs1 = (sbs, nil) /\
+    cmds2sbs cs2 = (nil, nbs).
+Proof.
+  induction cs; intros.
+    simpl in H. inversion H; subst.
+    exists nil. exists nil. auto.
+
+    simpl in H.
+    remember (isCallInst_dec a) as R.
+    remember (cmds2sbs cs) as R'.
+    destruct R.
+      destruct R'.
+        destruct l0.
+          inversion H; subst. clear H.
+          
+          destruct (@IHcs nil l1) as [cs1 [cs2 [J1 [J2 J3]]]]; subst; auto.
+          apply cmds2sbs_nil_inv in J2. subst.
+          exists nil. exists (a::cs2).
+          simpl. rewrite <- HeqR. 
+          simpl in HeqR'. rewrite <- HeqR'.
+          split; auto.
+
+       destruct s.
+       inversion H; subst. clear H.
+       destruct (@IHcs (mkSB NBs0 call_cmd0 call_cmd_isCall0::l0) nbs) as [cs1 [cs2 [J1 [J2 J3]]]]; subst; auto.
+       clear IHcs.
+       exists (a::cs1). exists cs2.
+       simpl. rewrite <- HeqR. rewrite J2. auto.
+    
+     destruct R'.
+     inversion H; subst. clear H.
+     destruct (@IHcs l0 nbs) as [cs1 [cs2 [J1 [J2 J3]]]]; subst; auto.
+     clear IHcs.
+     exists (a::cs1). exists cs2.
+     simpl. rewrite <- HeqR. rewrite J2. auto.
+Qed.
+
+Lemma cmds2sbs_cons_inv' : forall cs0 sb sbs' nbs,
+  cmds2sbs cs0 = (sb::sbs', nbs) ->
+  exists cs, exists cs',
+    cmds2sbs cs = (sb::nil, nil) /\
+    cmds2sbs cs' = (sbs', nbs) /\
+    cs0 = cs++cs'.
+Proof.
+  induction cs0; intros.
+    simpl in H. inversion H.
+
+    simpl in H.
+    remember (isCallInst_dec a) as R.
+    remember (cmds2sbs cs0) as R'.
+    destruct R.
+      destruct R'.
+        destruct l0.
+          inversion H.
+
+          destruct s. inversion H; subst. clear H.
+          destruct (@IHcs0 (mkSB NBs0 call_cmd0 call_cmd_isCall0) sbs' nbs) as [cs [cs' [J1 [J2 J3]]]]; subst; auto.
+          exists (a::cs). exists cs'.
+          split; auto.
+            simpl.
+            rewrite <- HeqR.
+            rewrite J1. auto.
+
+      destruct R'.
+      inversion H; subst. clear H.
+      destruct sbs'.
+        symmetry in HeqR'.
+        exists (a::nil). exists cs0.
+        simpl. rewrite <- HeqR. auto.
+
+        destruct (@IHcs0 s sbs' nbs) as [cs [cs' [J1 [J2 J3]]]]; subst; auto.
+        exists (a::nil). exists (cs++cs').
+        simpl. rewrite <- HeqR. auto.
+Qed.
+
+  
+Lemma cmds2nbs_app_inv : forall cs0 nbs1 nbs2,
+  cmds2sbs cs0 = (nil, nbs1++nbs2) ->
+  exists cs, exists cs',
+    cmds2sbs cs = (nil, nbs1) /\
+    cmds2sbs cs' = (nil, nbs2) /\
+    cs0 = cs++cs'.
+Proof.
+  induction cs0; intros.
+    simpl in H. inversion H.
+    symmetry in H1.
+    apply app_eq_nil in H1.
+    destruct H1; subst.
+    exists nil. exists nil. auto.
+
+    simpl in H.
+    remember (isCallInst_dec a) as R.
+    remember (cmds2sbs cs0) as R'.
+    destruct R.
+      destruct R'.
+        destruct l0.
+          inversion H.
+          apply cons_eq_app in H1.
+          destruct H1 as [[qs [J1 J2]] | [J1 J2]]; subst.
+            destruct (@IHcs0 qs nbs2) as [cs [cs' [J1 [J2 J3]]]]; subst; auto.
+            clear IHcs0.
+            exists (a::cs). exists cs'.
+            simpl. rewrite <- HeqR. rewrite J1. split; auto.
+
+            exists nil. exists (a::cs0). 
+            simpl. rewrite <- HeqR. rewrite <- HeqR'. split; auto.
+
+          destruct s. inversion H; subst.
+
+      destruct R'.
+      inversion H; subst. 
+Qed.
+
+Lemma nbranchs2cmds_app : forall nbs1 nbs2,
+  nbranchs2cmds (nbs1++nbs2) = nbranchs2cmds nbs1 ++ nbranchs2cmds nbs2.
+Proof.
+  induction nbs1; intros; auto.
+    simpl. destruct a. rewrite IHnbs1. auto.
+Qed.
+
+Lemma cmds_cons2nbranchs_inv : forall c cs' nbs,
+  cmds2nbranchs (c::cs') = Some nbs ->
+  exists nb, exists nbs',
+    cmd2nbranch c = Some nb /\
+    cmds2nbranchs cs' = Some nbs' /\
+    nbs = nb::nbs'.
+Proof.
+  intros.
+  simpl in H.
+  destruct (cmd2nbranch c); try solve [inversion H].
+  destruct (cmds2nbranchs cs'); inversion H; subst.
+  exists n. exists l0. auto.
+Qed.
+
+Lemma cmd2nbranch_Some_isCallInst : forall c nb,
+  cmd2nbranch c = Some nb ->
+  exists H, nb = mkNB c H.
+Proof.
+  intros.
+  unfold cmd2nbranch in H.
+  destruct nb.
+  destruct (isCallInst_dec c); inversion H; subst.
+    exists notcall0. auto. 
+Qed.
+
+(* wf *)
+Lemma wf_nbranchs__decomposes__app : forall nbs1 nbs2,
+  wf_nbranchs (nbs1++nbs2) ->
+  wf_nbranchs nbs1 /\ wf_nbranchs nbs2.
+Proof.
+  intros.
+  inversion H; subst.
+  apply cmds2nbs_app_inv in H0.
+  destruct H0 as [cs1 [cs2 [J1 [J2 J3]]]]; subst.
+  rewrite getCmdsIDs_app in H1.
+  apply NoDup_inv in H1.
+  destruct H1.
+  split; eapply wf_nbranchs_intro; eauto.
+Qed.
+
+Lemma wf_nbranchs__inv : forall nb nbs,
+  wf_nbranchs (nb::nbs) ->
+  wf_nbranchs nbs.
+Proof.
+  intros.
+  simpl_env in H.
+  apply wf_nbranchs__decomposes__app in H.
+  destruct H; auto.
+Qed.
+
+Lemma wf_nbranchs_nil : wf_nbranchs nil.
+Proof.
+  apply wf_nbranchs_intro with (cs:=nil); simpl; auto using NoDup_nil.
+Qed.
+
+Hint Resolve wf_nbranchs_nil.
+
+Lemma uniqCmds___wf_subblocks_wf_nbranchs : forall cs sbs nbs,
+  NoDup (getCmdsIDs cs) ->
+  cmds2sbs cs = (sbs, nbs) ->
+  wf_subblocks sbs /\ wf_nbranchs nbs.
+Proof.
+  induction cs; intros.
+    simpl in H0. inversion H0; subst.
+    split; auto using wf_nbranchs_nil.
+
+    simpl in *.
+    remember (cmds2sbs cs) as R.
+    destruct R as [sbs' nbs'].
+    remember (isCallInst_dec a) as R'.
+    destruct R'.
+      destruct sbs'.
+        inversion H0; subst. clear H0.
+        split; auto.
+          apply wf_nbranchs_intro with (cs:=a::cs); auto.
+            simpl.
+            rewrite <- HeqR'.
+            rewrite <- HeqR. auto.
+
+        destruct s. 
+        inversion H0; subst. clear H0.
+        inversion H; subst.
+        apply IHcs with (nbs0:=nbs)(sbs:=mkSB NBs0 call_cmd0 call_cmd_isCall0::sbs') in H3; auto.
+        destruct H3 as [H3 H4].
+        split; auto.
+          inversion H3; subst.
+          apply wf_subblocks_cons; auto.
+            apply wf_subblock_intro.
+
+            symmetry in HeqR.
+            apply cmds2sbs_cons_inv' in HeqR.
+            destruct HeqR as [cs1 [cs2 [Hcs1NBs0call0 [Hcs2sbs EQ]]]]; subst.
+            apply cmds2sb_inv in Hcs1NBs0call0.
+            destruct Hcs1NBs0call0 as [cs1' [call0 [EQ [Hcs1'nbs EQ']]]]; subst.
+            simpl in *.
+            simpl_env in H.
+            rewrite getCmdsIDs_app in H.
+            rewrite ass_app in H.
+            apply NoDup_inv in H. destruct H as [H _].
+            apply wf_nbranchs_intro with (cs:=a::cs1'); auto.
+              simpl.
+              rewrite <- HeqR'.
+              rewrite Hcs1'nbs. auto.
+
+      inversion H0; subst. clear H0.
+      simpl_env in H.
+      apply NoDup_inv in H. destruct H as [H1 H2].
+      apply IHcs with (sbs:=sbs')(nbs0:=nbs) in H2; auto.
+      destruct H2.
+      split; auto.
+        apply wf_subblocks_cons; auto.
+          apply wf_subblock_intro; auto.
+Qed.
+
+Lemma uniqBlock__wf_block : forall B,
+  uniqBlocks [B] -> wf_block B.
+Proof.
+  intros B HuniqBlocks.
+  unfold uniqBlocks in HuniqBlocks.
+  simpl in HuniqBlocks. destruct B.
+  destruct HuniqBlocks as [J1 J2].
+  remember (cmds2sbs c) as R.
+  destruct R as [sbs nbs].
+  simpl in J2. simpl_env in J2.
+  apply NoDup_inv in J2. destruct J2.
+  apply NoDup_inv in H0. destruct H0.
+  apply uniqCmds___wf_subblocks_wf_nbranchs with (sbs:=sbs)(nbs:=nbs) in H0; auto.
+  destruct H0.
+  apply wf_block_intro with (sbs:=sbs)(nbs:=nbs); auto.
+Qed.
+
+Lemma uniqBlocks__wf_block : forall lb n B,
+  uniqBlocks lb ->
+  nth_error lb n = Some B ->
+  wf_block B.
+Proof.
+  induction lb; intros.
+    apply nil_nth_error_Some__False in H0.
+    inversion H0.
+
+    apply nth_error_cons__inv in H0.
+    simpl_env in H. 
+    apply uniqBlocks_inv in H.
+    destruct H as [J1 J2].
+    destruct H0 as [EQ | [n' [EQ H0]]]; subst; eauto.
+      apply uniqBlock__wf_block; auto.
+Qed.
+
+Lemma uniqFdef__wf_block : forall fh lb n B,
+  uniqFdef (fdef_intro fh lb) ->
+  nth_error lb n = Some B ->
+  wf_block B.
+Proof.
+  intros.
+  unfold uniqFdef in H.
+  eapply uniqBlocks__wf_block; eauto.
+Qed.
+
+(* Properties of se *)
+
+Lemma se_cmd_uniq : forall smap0 sm0 sf0 se0 c,
+  uniq smap0 ->
+  uniq (STerms (se_cmd (mkSstate smap0 sm0 sf0 se0) c)).
+Proof.
+  intros smap0 sm0 sf0 se0 [c nocall] Huniq.
+  destruct c; simpl; 
+    try solve [
+      apply updateAddAL_uniq; auto | 
+      auto | 
+      inversion nocall].
+Qed.
+
+Lemma se_cmd_dom_mono : forall smap0 sm0 sf0 se0 c,
+  dom smap0 [<=] dom (STerms (se_cmd (mkSstate smap0 sm0 sf0 se0) c)).
+Proof.
+  intros smap0 sm0 sf0 se0 [c nocall].
+  assert (forall sm id0 st0, dom sm [<=] dom (updateAddAL sterm sm id0 st0)) as J.
+    intros. assert (J:=@updateAddAL_dom_eq _ sm id0 st0). fsetdec. 
+  destruct c; simpl; try solve [eauto using J| fsetdec|inversion nocall].
+Qed.
+
+Lemma _se_cmd_uniq : forall c sstate0,
+  uniq (STerms sstate0) ->
+  uniq (STerms (se_cmd sstate0 c)).
+Proof.
+  intros [c nocall] sstate0 Huniq.
+  destruct c; simpl; try solve [apply updateAddAL_uniq; auto | auto | inversion nocall].
+Qed.
+
+Lemma _se_cmds_uniq : forall cs sstate0,
+  uniq (STerms sstate0) ->
+  uniq (STerms (se_cmds sstate0 cs)).
+Proof.
+  induction cs; intros; simpl; auto using _se_cmd_uniq.
+Qed.
+
+Lemma se_cmds_uniq : forall cs smap0 sm0 sf0 se0,
+  uniq smap0 ->
+  uniq (STerms (se_cmds (mkSstate smap0 sm0 sf0 se0) cs)).
+Proof.
+  intros.
+  apply _se_cmds_uniq; auto. 
+Qed.
+
+Lemma se_cmds_init_uniq : forall cs,
+  uniq (STerms (se_cmds sstate_init cs)).
+Proof.
+  unfold sstate_init. intro. auto using se_cmds_uniq.
+Qed.
+
+Lemma se_cmds_rev_cons : forall cs c sstate0,
+  se_cmds sstate0 (cs++c::nil) = se_cmd (se_cmds sstate0 cs) c.
+Proof.
+  induction cs; intros; simpl; auto.
+Qed.
+
+Lemma se_cmds_app : forall cs cs' sstate0,
+  se_cmds sstate0 (cs++cs') = se_cmds (se_cmds sstate0 cs) cs'.
+Proof.
+  induction cs; intros; simpl; auto.
+Qed.
+
+Lemma se_cmds_cons : forall cs c sstate0,
+  se_cmds sstate0 ((c::nil)++cs) = se_cmds (se_cmd sstate0 c) cs.
+Proof.
+  induction cs; intros; simpl; auto.
+Qed.
+
+Lemma se_cmd_dom_upper : forall sstate0 c nc,
+  dom (STerms (se_cmd sstate0 (mkNB c nc))) [<=] dom (STerms sstate0) `union` {{getCmdID c}}.
+Proof.
+  intros [smap0 sm0 sf0 se0] c nc.
+  destruct c; simpl; try solve [rewrite updateAddAL_dom_eq; fsetdec | fsetdec | inversion nc].
+Qed.
+
+Lemma se_cmd_dom_mono' : forall sstate0 c,
+  dom (STerms sstate0) [<=] dom (STerms (se_cmd sstate0 c)).
+Proof.
+  intros [smap0 sm0 sf0 se0] c. 
+  simpl.
+  apply se_cmd_dom_mono; auto.
+Qed.
+
+Definition se_cmds_dom_mono_prop (cs:list nbranch) :=
+  forall smap0 sm0 sf0 se0,
+  dom smap0 [<=]
+    dom (STerms (se_cmds (mkSstate smap0 sm0 sf0 se0) cs)).
+
+Lemma se_cmds_dom_mono: forall cs, se_cmds_dom_mono_prop cs.
+Proof.
+  apply (@rev_ind nbranch); unfold se_cmds_dom_mono_prop; intros; simpl.
+    fsetdec.
+
+    rewrite se_cmds_rev_cons.
+    assert (J:=@se_cmd_dom_mono' (se_cmds (mkSstate smap0 sm0 sf0 se0) l0) x).
+    assert (J':=@H smap0 sm0 sf0 se0).
+    fsetdec.
+Qed.
+
+Lemma se_cmds_dom_mono' : forall sstate0 cs,
+  dom (STerms sstate0) [<=] dom (STerms (se_cmds sstate0 cs)).
+Proof.
+  intros [smap0 sm0 sf0 se0] cs. 
+  simpl.
+  apply se_cmds_dom_mono; auto.
+Qed.
+
+(* props of lookupSmap *)
+
+Lemma lookupSmap_in : forall sm id0 st0,
+  uniq sm ->
+  binds id0 st0 sm ->
+  lookupSmap sm id0 = st0.
+Proof.
+  induction sm; intros.
+    inversion H0.
+
+    destruct a.
+    simpl in *.
+    inversion H; subst.
+    destruct (@eq_dec id (@EqDec_eq_of_EqDec id EqDec_atom) id0 a); subst; simpl;
+      analyze_binds_uniq H0; auto.
+Qed.
+
+Lemma id2Sterm_in : forall sm id0 st0,
+  uniq sm ->
+  binds id0 st0 sm ->
+  value2Sterm sm (value_id id0) = st0.
+Proof.
+  intros. simpl. apply lookupSmap_in; auto.
+Qed.
+
+Lemma lookupSmap_notin : forall sm id0,
+  uniq sm ->
+  id0 `notin` dom sm ->
+  lookupSmap sm id0 = sterm_val (value_id id0).
+Proof.
+  induction sm; intros; simpl; auto.
+    destruct a.
+    simpl in *.
+    inversion H; subst.
+    destruct (@eq_dec id (@EqDec_eq_of_EqDec id EqDec_atom) id0 a); subst; simpl;
+      analyze_binds_uniq H0; auto.
+Qed.
+
+Lemma id2Sterm_notin : forall sm id0,
+  uniq sm ->
+  id0 `notin` dom sm ->
+  value2Sterm sm (value_id id0) = sterm_val (value_id id0).
+Proof.
+  intros. simpl. apply lookupSmap_notin; auto.
+Qed.
+
+Lemma const2Sterm : forall sm c,
+  value2Sterm sm (value_const c) = sterm_val (value_const c).
+Proof.
+  intros. auto.
+Qed.
+       
+Lemma lookupSmap_in_lookupAL : forall m id0,
+  id0 `in` dom m ->
+  lookupAL _ m id0 = Some (lookupSmap m id0).
+Proof.
+  induction m; intros id0 id0inm; simpl.
+    contradict id0inm; auto.
+
+    destruct a.
+    destruct (@eq_dec id (@EqDec_eq_of_EqDec id EqDec_atom) id0 a); subst.
+      destruct (@eq_dec atom (@EqDec_eq_of_EqDec atom EqDec_atom) a a); subst; simpl; auto.
+        contradict n; auto.
+      assert (id0 = a \/ id0 `in` dom m) as id0in. simpl in id0inm. fsetdec.
+      destruct id0in as [EQ | id0in]; subst.
+        contradict n; auto.
+        destruct (@eq_dec atom (@EqDec_eq_of_EqDec atom EqDec_atom) id0 a); subst; auto.
+          contradict n; auto.
+Qed.
+
+Lemma lookupSmap_updateAddAL_neq : forall m id0 id1 gv0,
+  id1 <> id0 ->
+  lookupSmap m id1 = lookupSmap (updateAddAL _ m id0 gv0) id1.
+Proof.
+  induction m; intros; simpl; auto.
+    destruct (@eq_dec id (EqDec_eq_of_EqDec id EqDec_atom) id1 id0); subst; auto.
+      contradict H; auto.
+
+    destruct a.
+      destruct (@eq_dec atom (@EqDec_eq_of_EqDec atom EqDec_atom) id1 id0); subst; simpl; auto.
+        contradict H; auto.
+        destruct (@eq_dec atom (@EqDec_eq_of_EqDec atom EqDec_atom) id1 a); subst; simpl; auto.
+          destruct (@eq_dec atom (@EqDec_eq_of_EqDec atom EqDec_atom) id0 a); subst; simpl; auto.
+            contradict H; auto.
+            destruct (@eq_dec id (@EqDec_eq_of_EqDec id EqDec_atom) a a); subst; simpl; auto.
+          destruct (@eq_dec atom (@EqDec_eq_of_EqDec atom EqDec_atom) id0 a); subst; simpl; auto.
+            destruct (@eq_dec id (@EqDec_eq_of_EqDec id EqDec_atom) id1 a); subst; simpl; auto.
+              contradict n; auto.
+            destruct (@eq_dec id (@EqDec_eq_of_EqDec id EqDec_atom) id1 a); subst; simpl; auto.
+Qed.   
+
+Lemma lookupSmap_updateAddAL_eq : forall m id0 gv0,
+  lookupSmap (updateAddAL _ m id0 gv0) id0 = gv0.
+Proof.
+  induction m; intros; simpl.
+    destruct (@eq_dec id (@EqDec_eq_of_EqDec id EqDec_atom) id0 id0); subst; simpl; auto.
+      contradict n; auto.  
+
+    destruct a.
+    destruct (@eq_dec atom (@EqDec_eq_of_EqDec atom EqDec_atom) id0 a); subst; simpl.
+      destruct (@eq_dec id (@EqDec_eq_of_EqDec id EqDec_atom) a a); subst; simpl; auto.
+        contradict n; auto.
+      destruct (@eq_dec id (@EqDec_eq_of_EqDec id EqDec_atom) id0 a); subst; simpl; auto.
+        contradict n; auto.
+Qed.
+
+Lemma lookupSmap_se_cmd_neq : forall c id' smap1 smem1 sframe1 seffects1 nc,
+  getCmdID c <> id' ->
+  lookupSmap (STerms (se_cmd (mkSstate smap1 smem1 sframe1 seffects1) (mkNB c nc))) id' =
+  lookupSmap smap1 id'.
+Proof.
+  destruct c; intros id' smap1 smem1 sframe1 seffects1 nc HnEQ; simpl;
+    try solve [rewrite <- lookupSmap_updateAddAL_neq; auto | inversion nc | auto].
+Qed.
+
+Lemma init_denotes_id : forall TD lc gl als Mem0,
+  sstate_denotes_state TD lc gl als Mem0 sstate_init lc als Mem0 trace_nil.
+Proof.
+  intros TD lc gl als Mem0.
+  split; auto.
+    split; intros; simpl in *; auto.
+      assert (id' `in` dom lc) as id'_in_lc. fsetdec.
+      apply indom_lookupAL_Some in id'_in_lc.
+      destruct id'_in_lc as [gv' id'_gv'_in_lc].
+      exists gv'. split; auto.
+Qed.
+
+(* props of denotes *)
+
+Lemma id_denotes_gv : forall id0 TD Mem0 gl lc,
+  id0 `in` dom lc ->
+  exists gv0,
+    sterm_denotes_genericvalue TD lc gl Mem0 (sterm_val (value_id id0)) gv0 /\
+    lookupAL _ lc id0 = Some gv0.
+Proof.
+  intros id0 TD Mem0 gl lc Hin.
+  apply indom_lookupAL_Some in Hin.
+  destruct Hin as [gv0 Hin].
+  exists gv0. split; auto.
+Qed.
+
+Lemma init_denotes_gvmap :forall TD lc gl Mem0,
+  uniq lc ->
+  smap_denotes_gvmap TD lc gl Mem0 nil lc.
+Proof.
+  intros TD lc gl Mem0 Uniqc.
+  unfold smap_denotes_gvmap.
+  split; intros; simpl; auto.
+    apply id_denotes_gv; auto. 
+      fsetdec.
+Qed.
+
+(* The denotational rules are determinastic. *)
+
+Definition sterm_denotes_genericvalue_det_prop TD lc gl Mem0 st0 gv1 
+  (sd:sterm_denotes_genericvalue TD lc gl Mem0 st0 gv1) :=
+  forall gv2,
+  sterm_denotes_genericvalue TD lc gl Mem0 st0 gv2 ->
+  gv1 = gv2.
+
+Definition sterms_denote_genericvalues_det_prop TD lc gl Mem0 sts0 gvs1
+  (ds:sterms_denote_genericvalues TD lc gl Mem0 sts0 gvs1) :=
+  forall gvs2,
+  sterms_denote_genericvalues TD lc gl Mem0 sts0 gvs2 ->
+  gvs1 = gvs2.
+
+Definition smem_denotes_mem_det_prop TD lc gl Mem0 st0 Mem1
+  (sd:smem_denotes_mem TD lc gl Mem0 st0 Mem1) :=
+  forall Mem2,
+  smem_denotes_mem TD lc gl Mem0 st0 Mem2 ->
+  Mem1 = Mem2.
+
+Lemma sdenotes_det : 
+  (forall TD lc gl Mem0 st0 gv1 sd, @sterm_denotes_genericvalue_det_prop TD lc gl Mem0 st0 gv1 sd) /\
+  (forall TD lc gl Mem0 sts0 gvs1 sd, @sterms_denote_genericvalues_det_prop TD lc gl Mem0 sts0 gvs1 sd) /\
+  (forall TD lc gl Mem0 st0 Mem1 sd, @smem_denotes_mem_det_prop TD lc gl Mem0 st0 Mem1 sd).
+Proof.
+(sd_mutind_cases
+  apply sd_mutind with
+    (P  := sterm_denotes_genericvalue_det_prop)
+    (P0 := sterms_denote_genericvalues_det_prop)
+    (P1 := smem_denotes_mem_det_prop) Case);
+  unfold sterm_denotes_genericvalue_det_prop, 
+         sterms_denote_genericvalues_det_prop, 
+         smem_denotes_mem_det_prop; intros.
+Case "sterm_val_denotes".
+  inversion H; subst.
+  rewrite e in H5. inversion H5; auto.
+Case "sterm_bop_denotes".
+  inversion H1; subst.
+  apply H in H11; subst.
+  apply H0 in H12; subst.
+  rewrite H13 in e.
+  inversion e; auto.
+Case "sterm_fbop_denotes".
+  inversion H1; subst.
+  apply H in H11; subst.
+  apply H0 in H12; subst.
+  rewrite H13 in e.
+  inversion e; auto.
+Case "sterm_extractvalue_denotes".
+  inversion H0; subst.
+  apply H in H9; subst.
+  rewrite H10 in e.
+  inversion e; auto.
+Case "sterm_insertvalue_denotes".
+  inversion H1; subst.
+  apply H in H12; subst.
+  apply H0 in H13; subst.
+  rewrite H14 in e.
+  inversion e; auto.
+Case "sterm_malloc_denotes".
+  inversion H1; subst.
+  rewrite e in H12. inversion H12; subst.
+  apply H in H10; subst.
+  apply H0 in H13; subst.
+  rewrite H14 in e0. inversion e0; auto.
+Case "sterm_alloca_denotes".
+  inversion H1; subst.
+  rewrite e in H12. inversion H12; subst.
+  apply H in H10; subst.
+  apply H0 in H13; subst.
+  rewrite H14 in e0. inversion e0; auto.
+Case "sterm_load_denotes".
+  inversion H1; subst.
+  apply H0 in H12; subst.
+  apply H in H11; subst.
+  rewrite e in H13. inversion H13; auto.
+Case "sterm_gep_denotes".
+  inversion H1; subst.
+  apply H in H11; subst.
+  apply H0 in H12; subst.
+  rewrite H13 in e. inversion e; auto.
+Case "sterm_trunc_denotes".
+  inversion H0; subst.
+  apply H in H10; subst.
+  rewrite H11 in e.
+  inversion e; auto.
+Case "sterm_ext_denotes".
+  inversion H0; subst.
+  apply H in H10; subst.
+  rewrite H11 in e.
+  inversion e; auto.
+Case "sterm_cast_denotes".
+  inversion H0; subst.
+  apply H in H10; subst.
+  rewrite H11 in e.
+  inversion e; auto.
+Case "sterm_icmp_denotes".
+  inversion H1; subst.
+  apply H in H11; subst.
+  apply H0 in H12; subst.
+  rewrite H13 in e. inversion e; auto.
+Case "sterm_fcmp_denotes".
+  inversion H1; subst.
+  apply H in H11; subst.
+  apply H0 in H12; subst.
+  rewrite H13 in e. inversion e; auto.
+Case "sterm_select_denotes".
+  inversion H2; subst.
+  apply H in H11; subst.
+  apply H0 in H13; subst.
+  apply H1 in H14; subst; auto.
+Case "sterms_nil_denote".
+  inversion H; auto.
+Case "sterms_cons_denote".
+  inversion H1; subst.
+  apply H in H8; subst.
+  apply H0 in H10; subst; auto.
+Case "smem_init_denotes".
+  inversion H; auto.
+Case "smem_malloc_denotes".
+  inversion H1; subst.
+  apply H in H10; subst. 
+  apply H0 in H13; subst. 
+  rewrite H12 in e. inversion e; subst.
+  rewrite H14 in e0. inversion e0; auto.
+Case "smem_free_denotes".
+  inversion H1; subst.
+  apply H in H9; subst. 
+  apply H0 in H11; subst. 
+  rewrite H12 in e. inversion e; auto.
+Case "smem_alloca_denotes".
+  inversion H1; subst.
+  apply H in H10; subst. 
+  apply H0 in H13; subst. 
+  rewrite H12 in e. inversion e; subst.
+  rewrite H14 in e0. inversion e0; auto.
+Case "smem_load_denotes".
+  inversion H0; subst.
+  apply H in H10; auto. 
+Case "smem_store_denotes".
+  inversion H2; subst.
+  apply H in H13; subst. 
+  apply H0 in H14; subst. 
+  apply H1 in H15; subst. 
+  rewrite H16 in e. inversion e; auto.
+Qed.
+
+Lemma sterm_denotes_genericvalue_det : forall TD lc gl Mem0 st0 gv1 gv2,
+  sterm_denotes_genericvalue TD lc gl Mem0 st0 gv1 ->
+  sterm_denotes_genericvalue TD lc gl Mem0 st0 gv2 ->
+  gv1 = gv2.
+Proof.
+  destruct sdenotes_det as [J _].
+  unfold sterm_denotes_genericvalue_det_prop in J.
+  eauto.
+Qed.
+
+Lemma sterms_denote_genericvalues_det : forall TD lc gl Mem0 sts0 gvs1 gvs2,
+  sterms_denote_genericvalues TD lc gl Mem0 sts0 gvs1 ->
+  sterms_denote_genericvalues TD lc gl Mem0 sts0 gvs2 ->
+  gvs1 = gvs2.
+Proof.
+  destruct sdenotes_det as [_ [J _]].
+  unfold sterms_denote_genericvalues_det_prop in J.
+  eauto.
+Qed.
+
+Lemma smem_denotes_mem_det : forall TD lc gl Mem0 st0 Mem1 Mem2,
+  smem_denotes_mem TD lc gl Mem0 st0 Mem1 ->
+  smem_denotes_mem TD lc gl Mem0 st0 Mem2 ->
+  Mem1 = Mem2.
+Proof.
+  destruct sdenotes_det as [_ [_ J]].
+  unfold smem_denotes_mem_det_prop in J.
+  eauto.
+Qed.
+
+Lemma sframe_denotes_frame_det : forall TD lc gl als Mem0 st0 als1 als2,
+  sframe_denotes_frame TD lc gl als Mem0 st0 als1 ->
+  sframe_denotes_frame TD lc gl als Mem0 st0 als2 ->
+  als1 = als2.
+Proof.
+  intros.
+  generalize dependent als2.
+  induction H; intros.
+    inversion H0; auto.
+
+    inversion H4; subst.
+    apply smem_denotes_mem_det with (Mem1:=Mem4) in H; auto; subst.
+    apply sterm_denotes_genericvalue_det with (gv1:=gv1) in H2; auto; subst.
+    rewrite H1 in H18. inversion H18; subst.
+    rewrite H20 in H3. inversion H3; subst.
+    apply IHsframe_denotes_frame in H17; subst; auto.
+Qed.
+
+Lemma seffects_denote_trace_det : forall ses tr1 tr2,
+  seffects_denote_trace ses tr1 ->
+  seffects_denote_trace ses tr2 ->
+  tr1 = tr2.
+Proof.
+  intros. 
+  inversion H; subst.
+  inversion H0; subst; auto.
+Qed.
+
+Lemma lookupSmap_inv : forall m id0 st0,
+  lookupSmap m id0 = st0 ->
+  (id0 `in` dom m /\ binds id0 st0 m) \/ 
+  (id0 `notin` dom m /\ st0 = sterm_val (value_id id0)).
+Proof.
+  induction m; intros id0 st0 HlkSmap; simpl in *.
+    right. auto.
+
+    destruct a.
+    destruct (@eq_dec id (@EqDec_eq_of_EqDec id EqDec_atom) id0 a); subst.
+      left. auto.
+
+      remember (lookupSmap m id0) as st0.
+      symmetry in Heqst0.
+      apply IHm in Heqst0.
+      destruct Heqst0 as [[id0in binds_id0_st0] | [id0notin EQ]]; subst; auto.
+Qed.
+
+
+Lemma sterm_val_denotes_in : forall TD lc gl Mem0 id0 gv,
+  sterm_denotes_genericvalue TD lc gl Mem0 (sterm_val (value_id id0)) gv ->
+  id0 `in` dom lc.
+Proof.
+  intros TD lc gl Mem0 id0 gv Hdenotes.
+  inversion Hdenotes; subst.
+  simpl in H4.
+  apply lookupAL_Some_indom in H4; auto.
+Qed.
+
+Lemma smap_denotes_gvmap_det : forall TD lc gl Mem0 smap0 lc1 lc2,
+  uniq smap0 ->
+  smap_denotes_gvmap TD lc gl Mem0 smap0 lc1 ->
+  smap_denotes_gvmap TD lc gl Mem0 smap0 lc2 ->
+  eqAL _ lc1 lc2.
+Proof.
+  intros TD lc gl Mem0 smap0 lc1 lc2 Uniq J1 J2.
+  destruct J1 as [J11 J12].
+  destruct J2 as [J21 J22].
+  intros id0.
+  remember (lookupAL _ lc1 id0) as ogv1.
+  remember (lookupAL _ lc2 id0) as ogv2.
+  destruct ogv1 as [gv1 | ].
+    symmetry in Heqogv1.
+    apply J12 in Heqogv1.
+    destruct (@AtomSetProperties.In_dec id0 (dom smap0)) as [id0_in_smap0 | id0_notin_smap0].
+      assert (id0 `in` dom smap0 `union` dom lc) as id0_in_smap0_lc. auto.
+      apply J21 in id0_in_smap0_lc.
+      destruct id0_in_smap0_lc as [gv' [id0_denotes_gv' id0_in_lc2]].
+      rewrite id0_in_lc2 in Heqogv2. inversion Heqogv2; subst.
+      apply sterm_denotes_genericvalue_det with (gv2:=gv1) in id0_denotes_gv'; auto.
+      subst. auto.
+      
+      apply lookupSmap_notin in id0_notin_smap0; auto.
+      rewrite id0_notin_smap0 in Heqogv1.
+      assert (id0_in_lc:=@sterm_val_denotes_in TD lc gl Mem0 id0 gv1 Heqogv1).
+      assert (id0 `in` dom smap0 `union` dom lc) as id0_in_smap0_lc. auto.
+      apply J21 in id0_in_smap0_lc.
+      destruct id0_in_smap0_lc as [gv' [id0_denotes_gv' id0_in_lc2]].
+      rewrite id0_in_lc2 in Heqogv2. inversion Heqogv2; subst.
+      rewrite id0_notin_smap0 in id0_denotes_gv'.
+      apply sterm_denotes_genericvalue_det with (gv2:=gv1) in id0_denotes_gv'; auto.
+      subst. auto.
+    
+  destruct ogv2 as [gv2 | ]; auto.
+    symmetry in Heqogv2.
+    apply J22 in Heqogv2.
+    destruct (@AtomSetProperties.In_dec id0 (dom smap0)) as [id0_in_smap0 | id0_notin_smap0].
+      assert (id0 `in` dom smap0 `union` dom lc) as id0_in_smap0_lc. auto.   
+      apply J11 in id0_in_smap0_lc.
+      destruct id0_in_smap0_lc as [gv' [id0_denotes_gv' id0_in_lc1]].
+      rewrite id0_in_lc1 in Heqogv1.
+      inversion Heqogv1.
+
+      apply lookupSmap_notin in id0_notin_smap0; auto.
+      rewrite id0_notin_smap0 in Heqogv2.
+      assert (id0_in_lc:=@sterm_val_denotes_in TD lc gl Mem0 id0 gv2 Heqogv2).
+      assert (id0 `in` dom smap0 `union` dom lc) as id0_in_smap0_lc. auto.
+      apply J11 in id0_in_smap0_lc.
+      destruct id0_in_smap0_lc as [gv' [id0_denotes_gv' id0_in_lc1]].
+      rewrite id0_in_lc1 in Heqogv1. inversion Heqogv1; subst.
+Qed.
+
+Lemma sstate_denotes_state_det : forall TD lc gl als Mem0 sstate0 lc1 als1 Mem1 tr1 lc2 als2 Mem2 tr2,
+  uniq (STerms sstate0) ->
+  sstate_denotes_state TD lc gl als Mem0 sstate0 lc1 als1 Mem1 tr1 ->
+  sstate_denotes_state TD lc gl als Mem0 sstate0 lc2 als2 Mem2 tr2 ->
+  eqAL _ lc1 lc2 /\ als1 = als2 /\ Mem1 = Mem2 /\ tr1 = tr2.
+Proof.
+  intros TD lc gl als Mem0 sstate0 lc1 als1 Mem1 tr1 lc2 als2 Mem2 tr2 Uniq J1 J2.
+  destruct J1 as [J11 [J12 [J13 J14]]].
+  destruct J2 as [J21 [J22 [J23 J24]]].
+  apply smem_denotes_mem_det with (Mem2:=Mem2) in J12; auto; subst.
+  apply sframe_denotes_frame_det with (als2:=als2) in J13; auto; subst.
+  apply seffects_denote_trace_det with (tr2:=tr2) in J14; auto; subst.
+  apply smap_denotes_gvmap_det with (lc2:=lc2) in J11; auto.
+Qed.
+
+Lemma smap_denotes_gvmap_eqEnv : forall TD lc gl Mem0 smap0 lc1 lc2,
+  smap_denotes_gvmap TD lc gl Mem0 smap0 lc1 ->
+  eqAL _ lc1 lc2 ->
+  smap_denotes_gvmap TD lc gl Mem0 smap0 lc2.
+Proof.
+  intros TD lc gl Mem0 smap0 lc1 lc2 [H1 H2] H3.
+  split; intros.
+    apply H1 in H.
+    destruct H as [gv' [st'_denotes_gv' id'_gv'_is_env1]].
+    exists gv'. rewrite <- H3.
+    split; auto.
+
+    rewrite <- H3 in H.
+    apply H2 in H; auto.
+Qed.
+
+(* p&p *)
+Lemma se_dbCmd_preservation : forall TD lc als gl Mem0 c lc' als' Mem' tr,
+  dbCmd TD gl lc als Mem0 c lc' als' Mem' tr ->
+  uniq lc ->
+  uniq lc'.
+Proof.
+  intros TD lc als gl Mem0 c lc' als' Mem' tr HdbCmd Uniqlc.
+  (dbCmd_cases (inversion HdbCmd) Case); subst; auto using updateAddAL_uniq.
+  Case "dbSelect".
+    destruct (isGVZero TD cond0); eauto using updateAddAL_uniq.
+Qed.
+
+Lemma se_dbCmds_preservation : forall TD lc als gl Mem0 cs lc' als' Mem' tr,
+  dbCmds TD gl lc als Mem0 cs lc' als' Mem' tr ->
+  uniq lc ->
+  uniq lc'.
+Proof.
+  intros TD lc als gl Mem0 cs lc' als' Mem' tr HdbCmd Uniqlc.
+  induction HdbCmd; auto. 
+    apply se_dbCmd_preservation in H; auto.
+Qed.
+
+Lemma se_dbTerminator_preservation : forall TD F B gl lc c B' lc' tr,
+  dbTerminator TD F gl B lc c B' lc' tr ->
+  uniq lc ->
+  uniqFdef F ->
+  blockInFdefB B F ->
+  uniq lc' /\ blockInFdefB B' F.
+Proof.
+  intros TD F gl B lc c B' lc' tr HdbTerminator Uniqlc UniqF Hblockin.
+  inversion HdbTerminator; subst.
+    destruct (isGVZero TD c0).
+      split; auto using switchToNewBasicBlock_uniq.
+        symmetry in H0.
+        apply lookupBlockViaLabelFromFdef_inv in H0; auto.
+        destruct H0; auto.
+
+      split; auto using switchToNewBasicBlock_uniq.
+        symmetry in H0.
+        apply lookupBlockViaLabelFromFdef_inv in H0; auto.
+        destruct H0; auto.
+
+    symmetry in H.
+    apply lookupBlockViaLabelFromFdef_inv in H; auto.
+    destruct H.
+    split; auto using switchToNewBasicBlock_uniq.
+Qed.
+
+Definition se_dbCall_preservation_prop S TD Ps fs gl lc Mem0 call0 lc' Mem' tr
+  (db:dbCall S TD Ps fs gl lc Mem0 call0 lc' Mem' tr) :=
+  forall los nts,
+  uniq lc ->
+  uniqSystem S ->
+  moduleInSystem (module_intro los nts Ps) S ->
+  TD = (los, nts) ->
+  uniq lc' .
+Definition se_dbSubblock_preservation_prop S TD Ps fs gl lc als Mem cs lc' als' Mem' tr
+  (db:dbSubblock S TD Ps fs gl lc als Mem cs lc' als' Mem' tr) :=
+  forall los nts,
+  uniq lc ->
+  uniqSystem S ->
+  moduleInSystem (module_intro los nts Ps) S ->
+  TD = (los, nts) ->
+  uniq lc'.
+Definition se_dbSubblocks_preservation_prop S TD Ps fs gl lc als Mem cs lc' als' Mem' tr
+  (db:dbSubblocks S TD Ps fs gl lc als Mem cs lc' als' Mem' tr) :=
+  forall los nts,
+  uniq lc ->
+  uniqSystem S ->
+  moduleInSystem (module_intro los nts Ps) S ->
+  TD = (los, nts) ->
+  uniq lc'.
+Definition se_dbBlock_preservation_prop S TD Ps fs gl F arg state1 state2 tr
+  (db:dbBlock S TD Ps fs gl F arg state1 state2 tr) :=
+  forall B1 lc als Mem B1' lc' als' Mem' los nts,
+  state1 = mkState (mkEC B1 lc als) Mem ->
+  state2 = mkState (mkEC B1' lc' als') Mem' ->
+  uniq lc ->
+  uniqSystem S ->
+  blockInSystemModuleFdef B1 S (module_intro los nts Ps) F ->
+  TD = (los, nts) ->
+  uniq lc' /\ 
+  blockInSystemModuleFdef B1' S (module_intro los nts Ps) F.
+Definition se_dbBlocks_preservation_prop S TD Ps fs gl F lp state1 state2 tr
+  (db:dbBlocks S TD Ps fs gl F lp state1 state2 tr) :=
+  forall B1 lc als Mem B1' lc' als' Mem' los nts,
+  state1 = (mkState (mkEC B1 lc als) Mem) ->
+  state2 = (mkState (mkEC B1' lc' als') Mem') ->
+  uniq lc ->
+  uniqSystem S ->
+  blockInSystemModuleFdef B1 S (module_intro los nts Ps) F ->
+  TD = (los, nts) ->
+  uniq lc' /\ 
+  blockInSystemModuleFdef B1' S (module_intro los nts Ps) F.
+Definition se_dbFdef_preservation_prop fv rt lp S TD Ps lc gl fs Mem lc' als' Mem' B' Rid oResult tr
+  (db:dbFdef fv rt lp S TD Ps lc gl fs Mem lc' als' Mem' B' Rid oResult tr) :=
+  forall fid la lb los nts,
+  lookupFdefViaGV TD Ps gl lc fs fv = Some (fdef_intro (fheader_intro rt fid la) lb) ->
+  uniq lc ->
+  uniqSystem S ->
+  moduleInSystem (module_intro los nts Ps) S ->
+  TD = (los, nts) ->
+  uniq lc' /\ 
+  blockInSystemModuleFdef B' S (module_intro los nts Ps) (fdef_intro (fheader_intro rt fid la) lb).
+
+Lemma se_db_preservation :
+  (forall S TD Ps fs gl lc Mem0 call0 lc' Mem' tr db, 
+     se_dbCall_preservation_prop S TD Ps fs gl lc Mem0 call0 lc' Mem' tr db) /\
+  (forall S TD Ps fs gl lc als Mem sb lc' als' Mem' tr db,
+     se_dbSubblock_preservation_prop S TD Ps fs gl lc als Mem sb lc' als' Mem' tr db) /\
+  (forall S TD Ps fs gl lc als Mem sbs lc' als' Mem' tr db,
+     se_dbSubblocks_preservation_prop S TD Ps fs gl lc als Mem sbs lc' als' Mem' tr db) /\
+  (forall S TD Ps fs gl F arg state1 state2 tr db,
+     se_dbBlock_preservation_prop S TD Ps fs gl F arg state1 state2 tr db) /\
+  (forall S TD Ps fs gl F lp state1 state2 tr db,
+     se_dbBlocks_preservation_prop S TD Ps fs gl F lp state1 state2 tr db) /\
+  (forall fid rt lp S TD Ps lc gl fs Mem lc' als' Mem' B' Rid oResult tr db,
+     se_dbFdef_preservation_prop fid rt lp S TD Ps lc gl fs Mem lc' als' Mem' B' Rid oResult tr db).
+Proof.
+(db_mutind_cases
+  apply db_mutind with
+    (P  := se_dbCall_preservation_prop)
+    (P0 := se_dbSubblock_preservation_prop)
+    (P1 := se_dbSubblocks_preservation_prop)
+    (P2 := se_dbBlock_preservation_prop)
+    (P3 := se_dbBlocks_preservation_prop)
+    (P4 := se_dbFdef_preservation_prop) Case);
+  unfold se_dbCall_preservation_prop, 
+         se_dbSubblock_preservation_prop, se_dbSubblocks_preservation_prop,
+         se_dbBlock_preservation_prop, se_dbBlocks_preservation_prop,
+         se_dbFdef_preservation_prop; intros; subst; eauto.
+Case "dbCall_internal".
+  inversion d; subst.
+    eapply H in H3; eauto. clear H.
+    destruct H3 as [Huniqlc' Hblockin].
+    unfold callUpdateLocals.
+    destruct noret0; auto.
+      destruct (rt=t=typ_void); auto.
+        destruct (getOperandValue (los, nts) Result lc' gl); auto.
+          apply updateAddAL_uniq; auto.
+
+    eapply H in H3; eauto. clear H.
+    destruct H3 as [Huniqlc' Hblockin].
+    unfold callUpdateLocals.
+    destruct noret0; auto.
+      destruct (rt=t=typ_void); auto.
+
+Case "dbCall_external".
+  unfold exCallUpdateLocals.
+  destruct noret0; auto.
+  destruct (rt=t=typ_void); auto.
+  destruct oresult; auto.
+  apply updateAddAL_uniq; auto.
+
+Case "dbSubblock_intro".
+  apply se_dbCmds_preservation in d; eauto.
+ 
+Case "dbBlock_intro".
+  inversion H0; subst. clear H0.
+  inversion H1; subst. clear H1.
+  apply blockInSystemModuleFdef_inv in H4.
+  destruct H4 as [Hblockin [Hinproducts [Hmodulein Hproductin]]].
+  eapply H in H2; eauto.
+  apply se_dbCmds_preservation in d0; auto.
+  assert (uniqFdef F) as uniqF.
+    apply uniqSystem__uniqFdef in Hproductin; auto.
+  apply se_dbTerminator_preservation in d1; auto.
+  destruct d1 as [uniqc' B1inF].
+  split; auto using blockInSystemModuleFdef_intro.
+
+Case "dbBlocks_nil".
+  inversion H0; subst. clear H0.
+  split; auto.
+ 
+Case "dbBlocks_cons".
+  inversion d; subst.
+  assert (J:=H4).
+  eapply H with (B1:=block_intro l0 ps (cs++cs') tmn)(lc0:=lc)(als0:=als)(Mem:=Mem0) 
+               (B1':=B')(lc':=lc4)(als':=als3)(Mem':=Mem3) in J; eauto.
+  clear H.
+  destruct J as [uniqc4 B'in].
+  eapply H0; eauto.
+
+Case "dbFdef_func".
+  rewrite e in H1. inversion H1; subst. clear H1.
+  apply entryBlockInSystemBlockFdef' with (los:=los)(nts:=nts)(Ps:=Ps)(S:=S)(fv:=fv)(gl:=gl)(lc:=lc)(fs:=fs) in e0; auto.
+  apply H with (B1:=block_intro l1 ps1 cs1 tmn1)(lc0:=initLocals la0 (params2GVs (los, nts) lp lc gl))(als:=nil)(Mem:=Mem0)
+               (B1':=block_intro l2 ps2 (cs21++cs22) (insn_return rid rt Result))(lc':=lc1)(als':=als1)(Mem':=Mem1) in e0; auto using initLocals_uniq.
+  clear H. destruct e0 as [uniqc1 Bin].
+  eapply H0 in uniqc1; eauto. clear H0.
+  apply se_dbCmds_preservation in d1; auto.
+
+Case "dbFdef_proc".
+  rewrite e in H1. inversion H1; subst. clear H1.
+  apply entryBlockInSystemBlockFdef' with (los:=los)(nts:=nts)(Ps:=Ps)(S:=S)(fv:=fv)(gl:=gl)(lc:=lc)(fs:=fs) in e0; auto.
+  apply H with (B1:=block_intro l1 ps1 cs1 tmn1)(lc0:=initLocals la0 (params2GVs (los, nts) lp lc gl))(als:=nil)(Mem:=Mem0)
+               (B1':=block_intro l2 ps2 (cs21++cs22) (insn_return_void rid))(lc':=lc1)(als':=als1)(Mem':=Mem1) in e0; auto using initLocals_uniq.
+  clear H. destruct e0 as [uniqc1 Bin].
+  eapply H0 in uniqc1; eauto. clear H0.
+  apply se_dbCmds_preservation in d1; auto.
+Qed.
+
+Lemma se_dbCall_preservation : forall S los nts Ps fs lc gl Mem0 call0 lc' Mem' tr,
+  dbCall S (los, nts) Ps fs gl lc Mem0 call0 lc' Mem' tr ->
+  uniq lc ->
+  uniqSystem S ->
+  moduleInSystem (module_intro los nts Ps) S ->
+  uniq lc' .
+Proof.
+  intros.
+  destruct se_db_preservation as [J _].
+  unfold se_dbCall_preservation_prop in J. eauto.
+Qed.
+
+Lemma se_dbSubblock_preservation : forall S los nts Ps fs gl lc als Mem cs lc' als' Mem' tr,
+  dbSubblock S (los, nts) Ps fs gl lc als Mem cs lc' als' Mem' tr ->
+  uniq lc ->
+  uniqSystem S ->
+  moduleInSystem (module_intro los nts Ps) S ->
+  uniq lc'.
+Proof.
+  intros.
+  destruct se_db_preservation as [_ [J _]].
+  unfold se_dbSubblock_preservation_prop in J. eauto.
+Qed.
+
+Lemma se_dbSubblocks_preservation : forall S los nts Ps fs gl lc als Mem cs lc' als' Mem' tr,
+  dbSubblocks S (los, nts) Ps fs gl lc als Mem cs lc' als' Mem' tr ->
+  uniq lc ->
+  uniqSystem S ->
+  moduleInSystem (module_intro los nts Ps) S ->
+  uniq lc'.
+Proof.
+  intros.
+  destruct se_db_preservation as [_ [_ [J _]]].
+  unfold se_dbSubblocks_preservation_prop in J. eauto.
+Qed.
+
+Lemma se_dbBlock_preservation : forall S los nts Ps fs gl F arg tr B1 lc als Mem B1' lc' als' Mem',
+  dbBlock S (los, nts)  Ps fs gl F arg 
+    (mkState (mkEC B1 lc als) Mem) 
+    (mkState (mkEC B1' lc' als') Mem') tr ->
+  uniq lc ->
+  uniqSystem S ->
+  blockInSystemModuleFdef B1 S (module_intro los nts Ps) F ->
+  uniq lc' /\ 
+  blockInSystemModuleFdef B1' S (module_intro los nts Ps) F.
+Proof.
+  intros.
+  destruct se_db_preservation as [_ [_ [_ [J _]]]].
+  unfold se_dbBlock_preservation_prop in J. eauto.
+Qed.
+
+Lemma se_dbBlocks_preservation : forall S los nts Ps fs gl F lp tr B1 lc als Mem B1' lc' als' Mem',
+  dbBlocks S (los, nts) Ps fs gl F lp 
+    (mkState (mkEC B1 lc als) Mem)
+    (mkState (mkEC B1' lc' als') Mem') tr ->
+  uniq lc ->
+  uniqSystem S ->
+  blockInSystemModuleFdef B1 S (module_intro los nts Ps) F ->
+  uniq lc' /\ 
+  blockInSystemModuleFdef B1' S (module_intro los nts Ps) F.
+Proof.
+  intros.
+  destruct se_db_preservation as [_ [_ [_ [_ [J _]]]]].
+  unfold se_dbBlocks_preservation_prop in J. eauto.
+Qed.
+
+Lemma se_dbFdef_preservation : forall fv rt lp S los nts Ps lc gl fs Mem lc' als' Mem' B' Rid oResult tr fid la lb,
+  dbFdef fv rt lp S (los, nts) Ps lc gl fs Mem lc' als' Mem' B' Rid oResult tr ->
+  lookupFdefViaGV (los, nts) Ps gl lc fs fv = Some (fdef_intro (fheader_intro rt fid la) lb) ->
+  uniq lc ->
+  uniqSystem S ->
+  moduleInSystem (module_intro los nts Ps) S ->
+  uniq lc' /\ 
+  blockInSystemModuleFdef B' S (module_intro los nts Ps) (fdef_intro (fheader_intro rt fid la) lb).
+Proof.
+  intros.
+  destruct se_db_preservation as [_ [_ [_ [_ [_ J]]]]].
+  unfold se_dbFdef_preservation_prop in J. eauto.
+Qed.
+
+(* eqEnv *)
+Lemma dbCmd_eqEnv : forall TD c lc1 als1 gl Mem1 lc2 als2 Mem2 tr lc1',
+  dbCmd TD gl lc1 als1 Mem1 c lc2 als2 Mem2 tr ->
+  eqAL _ lc1 lc1' ->
+  exists lc2', 
+    dbCmd TD gl lc1' als1 Mem1 c lc2' als2 Mem2 tr /\
+    eqAL _ lc2 lc2'.
+Proof.
+  intros TD c lc1 als1 gl Mem1 lc2 als2 Mem2 tr lc1' HdbCmd HeqEnv.
+  (dbCmd_cases (inversion HdbCmd) Case); subst.
+Case "dbBop".
+  assert (HupdateEnv:=HeqEnv).
+  exists (updateAddAL _ lc1' id0 gv3).
+  rewrite BOP_eqAL with (lc2:=lc1') in H; auto.
+  split; eauto using eqAL_updateAddAL.
+
+Case "dbFBop".
+  assert (HupdateEnv:=HeqEnv).
+  exists (updateAddAL _ lc1' id0 gv3).
+  rewrite FBOP_eqAL with (lc2:=lc1') in H; auto.
+  split; eauto using eqAL_updateAddAL.
+
+Case "dbExtractValue".
+  assert (HupdateEnv:=HeqEnv).
+  exists (updateAddAL _ lc1' id0 gv').
+  rewrite getOperandValue_eqAL with (lc2:=lc1') in H; auto. 
+  split; eauto using eqAL_updateAddAL.
+  
+Case "dbInsertValue".
+  assert (HupdateEnv:=HeqEnv).
+  exists (updateAddAL _ lc1' id0 gv'').
+  rewrite getOperandValue_eqAL with (lc2:=lc1') in H; auto. 
+  rewrite getOperandValue_eqAL with (lc2:=lc1') in H0; auto. 
+  split; eauto using eqAL_updateAddAL.
+
+Case "dbMalloc".
+  assert (HupdateEnv:=HeqEnv).
+  exists (updateAddAL _ lc1' id0 (blk2GV TD mb)).
+  rewrite getOperandValue_eqAL with (lc2:=lc1') in H0; auto. 
+  split; eauto using eqAL_updateAddAL.
+
+Case "dbFree".
+  exists lc1'.
+  rewrite getOperandValue_eqAL with (lc2:=lc1') in H; auto. 
+  split; eauto.
+
+Case "dbAlloca".
+  assert (HupdateEnv:=HeqEnv).
+  exists (updateAddAL _ lc1' id0 (blk2GV TD mb)).
+  rewrite getOperandValue_eqAL with (lc2:=lc1') in H0; auto. 
+  split; eauto using eqAL_updateAddAL.
+
+Case "dbLoad".
+  assert (HupdateEnv:=HeqEnv).
+  exists (updateAddAL _ lc1' id0 gv).
+  rewrite getOperandValue_eqAL with (lc2:=lc1') in H; auto. 
+  split; eauto using eqAL_updateAddAL.
+
+Case "dbStore".
+  exists lc1'.
+  rewrite getOperandValue_eqAL with (lc2:=lc1') in H; auto. 
+  rewrite getOperandValue_eqAL with (lc2:=lc1') in H0; auto. 
+  split; eauto using eqAL_updateAddAL.
+
+Case "dbGEP".
+  assert (HupdateEnv:=HeqEnv).
+  exists (updateAddAL _ lc1' id0 mp').
+  rewrite getOperandValue_eqAL with (lc2:=lc1') in H; auto. 
+  rewrite values2GVs_eqAL with (lc2:=lc1') in H0; auto. 
+(* rewrite GEP_eqAL with (lc2:=lc1') in H0; auto. *)
+  split; eauto using eqAL_updateAddAL.
+
+Case "dbTrunc".
+  assert (HupdateEnv:=HeqEnv).
+  exists (updateAddAL _ lc1' id0 gv2).
+  rewrite TRUNC_eqAL with (lc2:=lc1') in H; auto.
+  split; eauto using eqAL_updateAddAL.
+
+Case "dbExt".
+  assert (HupdateEnv:=HeqEnv).
+  exists (updateAddAL _ lc1' id0 gv2).
+  rewrite EXT_eqAL with (lc2:=lc1') in H; auto.
+  split; eauto using eqAL_updateAddAL.
+
+Case "dbCast".
+  assert (HupdateEnv:=HeqEnv).
+  exists (updateAddAL _ lc1' id0 gv2).
+  rewrite CAST_eqAL with (lc2:=lc1') in H; auto.
+  split; eauto using eqAL_updateAddAL.
+
+Case "dbIcmp".
+  assert (HupdateEnv:=HeqEnv).
+  exists (updateAddAL _ lc1' id0 gv3).
+  rewrite ICMP_eqAL with (lc2:=lc1') in H; auto.
+  split; eauto using eqAL_updateAddAL.
+
+Case "dbFcmp".
+  assert (HupdateEnv:=HeqEnv).
+  exists (updateAddAL _ lc1' id0 gv3).
+  rewrite FCMP_eqAL with (lc2:=lc1') in H; auto.
+  split; eauto using eqAL_updateAddAL.
+
+Case "dbSelect".
+  rewrite getOperandValue_eqAL with (lc2:=lc1') in H; auto. 
+  rewrite getOperandValue_eqAL with (lc2:=lc1') in H0; auto. 
+  rewrite getOperandValue_eqAL with (lc2:=lc1') in H1; auto. 
+  assert (HupdateEnv:=HeqEnv).
+  exists (if isGVZero TD cond0 then updateAddAL _ lc1' id0 gv2 else updateAddAL _ lc1' id0 gv1).
+  split; auto.
+    destruct (isGVZero TD cond0); auto using eqAL_updateAddAL.
+Qed.
+
+Lemma dbCmds_eqEnv : forall TD cs lc1 als1 gl Mem1 lc2 als2 Mem2 tr lc1',
+  dbCmds TD gl lc1 als1 Mem1 cs lc2 als2 Mem2 tr ->
+  eqAL _ lc1 lc1' ->
+  exists lc2', 
+    dbCmds TD gl lc1' als1 Mem1 cs lc2' als2 Mem2 tr /\
+    eqAL _ lc2 lc2'.
+Proof.
+  intros TD cs lc1 als1 gl Mem1 lc2 als2 Mem2 tr lc1' HdbCmds HeqEnv.
+  generalize dependent lc1'.
+  induction HdbCmds; intros.
+    exists lc1'. split; auto.
+
+    apply dbCmd_eqEnv with (lc1':=lc1') in H; auto.
+    destruct H as [lc2' [HdbCmd HeqEnv']].
+    apply IHHdbCmds in HeqEnv'; auto.
+    destruct HeqEnv' as [lc3' [HdbCmds' HeqEnv'']].
+    exists lc3'.
+    split; eauto.
+Qed.
+
+Lemma dbTerminator_eqEnv : forall TD F gl lc1 tmn lc2 tr lc1' B B',
+  dbTerminator TD F gl B lc1 tmn B' lc2 tr ->
+  eqAL _ lc1 lc1' ->
+  exists lc2',
+    dbTerminator TD F gl B lc1' tmn B' lc2' tr /\
+    eqAL _ lc2 lc2'.
+Proof.
+  intros TD F gl lc1 tmn lc2 tr lc1' B B' HdbTerminator HeqAL.
+  inversion HdbTerminator; subst.
+    exists (switchToNewBasicBlock TD (block_intro l' ps' sbs' tmn') B gl lc1').
+    split.
+      apply dbBranch with (c:=c); auto.
+        erewrite <- getOperandValue_eqAL; eauto.
+      apply eqAL_switchToNewBasicBlock; auto.     
+  
+    exists (switchToNewBasicBlock TD (block_intro l' ps' sbs' tmn') B gl lc1').
+    split.
+      apply dbBranch_uncond; auto.
+      apply eqAL_switchToNewBasicBlock; auto.
+Qed.     
+
+Definition dbCall_eqEnv_prop S TD Ps fs gl lc1 Mem0 call0 lc2 Mem' tr
+  (db:dbCall S TD Ps fs gl lc1 Mem0 call0 lc2 Mem' tr) := 
+  forall lc1',
+  eqAL _ lc1 lc1' ->
+  exists lc2',
+    dbCall S TD Ps fs gl lc1' Mem0 call0 lc2' Mem' tr /\
+    eqAL _ lc2 lc2'.
+Definition dbSubblock_eqEnv_prop S TD Ps fs gl lc1 als Mem cs lc2 als' Mem' tr
+  (db:dbSubblock S TD Ps fs gl lc1 als Mem cs lc2 als' Mem' tr) :=
+  forall lc1',
+  eqAL _ lc1 lc1' ->
+  exists lc2',
+    dbSubblock S TD Ps fs gl lc1' als Mem cs lc2' als' Mem' tr /\
+    eqAL _ lc2 lc2'.
+Definition dbSubblocks_eqEnv_prop S TD Ps fs gl lc1 als Mem cs lc2 als' Mem' tr
+  (db:dbSubblocks S TD Ps fs gl lc1 als Mem cs lc2 als' Mem' tr) :=
+  forall lc1',
+  eqAL _ lc1 lc1' ->
+  exists lc2',
+    dbSubblocks S TD Ps fs gl lc1' als Mem cs lc2' als' Mem' tr /\
+    eqAL _ lc2 lc2'.
+Definition dbBlock_eqEnv_prop S TD Ps fs gl F arg state1 state2 tr
+  (db:dbBlock S TD Ps fs gl F arg state1 state2 tr) :=
+  forall B1 lc1 als Mem B1' lc2 als' Mem' lc1',
+  state1 = mkState (mkEC B1 lc1 als) Mem ->
+  state2 = mkState (mkEC B1' lc2 als') Mem' ->
+  eqAL _ lc1 lc1' ->
+  exists lc2',
+    dbBlock S TD Ps fs gl F arg 
+     (mkState (mkEC B1 lc1' als) Mem) 
+     (mkState (mkEC B1' lc2' als') Mem') 
+     tr /\
+    eqAL _ lc2 lc2'.
+Definition dbBlocks_eqEnv_prop S TD Ps fs gl F lp state1 state2 tr
+  (db:dbBlocks S TD Ps fs gl F lp state1 state2 tr) :=
+  forall B1 lc1 als Mem B1' lc2 als' Mem' lc1',
+  state1 = mkState (mkEC B1 lc1 als) Mem ->
+  state2 = mkState (mkEC B1' lc2 als') Mem' ->
+  eqAL _ lc1 lc1' ->
+  exists lc2',
+    dbBlocks S TD Ps fs gl F lp 
+     (mkState (mkEC B1 lc1' als) Mem) 
+     (mkState (mkEC B1' lc2' als') Mem') 
+     tr /\
+    eqAL _ lc2 lc2'.
+Definition dbFdef_eqEnv_prop fv rt lp S TD Ps lc1 gl fs Mem lc2 als' Mem' B' Rid oResult tr
+  (db:dbFdef fv rt lp S TD Ps lc1 gl fs Mem lc2 als' Mem' B' Rid oResult tr) :=
+  forall fid la lb lc1',
+  lookupFdefViaGV TD Ps gl lc1 fs fv = Some (fdef_intro (fheader_intro rt fid la) lb) ->
+  eqAL _ lc1 lc1' ->
+  exists lc2',
+    dbFdef fv rt lp S TD Ps lc1' gl fs Mem lc2' als' Mem' B' Rid oResult tr /\
+    eqAL _ lc2 lc2'.
+
+Lemma db_eqEnv :
+  (forall S TD Ps fs gl lc Mem0 call0 lc' Mem' tr db, 
+     dbCall_eqEnv_prop S TD Ps fs gl lc Mem0 call0 lc' Mem' tr db) /\
+  (forall S TD Ps fs gl lc als Mem sb lc' als' Mem' tr db,
+     dbSubblock_eqEnv_prop S TD Ps fs gl lc als Mem sb lc' als' Mem' tr db) /\
+  (forall S TD Ps fs gl lc als Mem sbs lc' als' Mem' tr db,
+     dbSubblocks_eqEnv_prop S TD Ps fs gl lc als Mem sbs lc' als' Mem' tr db) /\
+  (forall S TD Ps fs gl F arg state1 state2 tr db,
+     dbBlock_eqEnv_prop S TD Ps fs gl F arg state1 state2 tr db) /\
+  (forall S TD Ps fs gl F lp state1 state2 tr db,
+     dbBlocks_eqEnv_prop S TD Ps fs gl F lp state1 state2 tr db) /\
+  (forall fid rt lp S TD Ps lc gl fs Mem lc' als' Mem' B' Rid oResult tr db,
+     dbFdef_eqEnv_prop fid rt lp S TD Ps lc gl fs Mem lc' als' Mem' B' Rid oResult tr db).
+Proof.
+(db_mutind_cases
+  apply db_mutind with
+    (P  := dbCall_eqEnv_prop)
+    (P0 := dbSubblock_eqEnv_prop)
+    (P1 := dbSubblocks_eqEnv_prop)
+    (P2 := dbBlock_eqEnv_prop)
+    (P3 := dbBlocks_eqEnv_prop)
+    (P4 := dbFdef_eqEnv_prop) Case);
+  unfold dbCall_eqEnv_prop, 
+         dbSubblock_eqEnv_prop, dbSubblocks_eqEnv_prop,
+         dbBlock_eqEnv_prop, dbBlocks_eqEnv_prop,
+         dbFdef_eqEnv_prop; intros; subst; auto.
+Case "dbCall_internal".
+  inversion d; subst.
+    apply H with (lc1':=lc1') in H1; auto. clear H.
+    destruct H1 as [lc2' [HdbBlocks HeqEnv]].
+    exists (callUpdateLocals TD noret0 rid rt (Some Result) lc1' lc2' gl).
+    split; eauto using dbCall_internal, eqAL_callUpdateLocals.
+
+    apply H with (lc1':=lc1') in H1; auto. clear H.
+    destruct H1 as [lc2' [HdbBlocks HeqEnv]].
+    exists (callUpdateLocals TD noret0 rid rt None lc1' lc2' gl).
+    split; eauto using dbCall_internal, eqAL_callUpdateLocals.
+
+Case "dbCall_external".
+  exists (exCallUpdateLocals noret0 rid rt oresult lc1').
+  split; eauto using eqAL_exCallUpdateLocals.
+    eapply dbCall_external; eauto.
+      erewrite eqAL_lookupExFdecViaGV; eauto using eqAL_sym.
+
+    rewrite <- eqAL_params2GVs with (lc:=lc); auto.
+
+Case "dbSubblock_intro".
+  apply dbCmds_eqEnv with (lc1':=lc1') in d; auto.
+  destruct d as [lc2' [HdbCmds HeqEnv2]].
+  apply H in HeqEnv2. clear H.
+  destruct HeqEnv2 as [lc3' [HdbCall HeqEnv3]].
+  exists lc3'.
+  split; eauto.
+
+Case "dbSubblocks_nil".
+  exists lc1'. split; auto.
+ 
+Case "dbSubblocks_cons".
+  apply H in H1. clear H.
+  destruct H1 as [lc2' [HdbSubblock Heq2]].
+  apply H0 in Heq2. clear H0.
+  destruct Heq2 as [lc3' [HdbSubblocks Heq3]].
+  exists lc3'. split; eauto.
+
+Case "dbBlock_intro".
+  inversion H0; subst. clear H0.
+  inversion H1; subst. clear H1.
+  apply H in H2. clear H.
+  destruct H2 as [lc2' [HdbSubblocks Heq2]].
+  apply dbCmds_eqEnv with (lc1':=lc2') in d0; auto.
+  destruct d0 as [lc3' [HdbCmds Heq3]].
+  apply dbTerminator_eqEnv with (lc1':=lc3') in d1; auto.
+  destruct d1 as [lc5' [HdbTerminator Heq5]].
+  exists lc5'. split; eauto.
+
+Case "dbBlocks_nil".
+  inversion H0; subst. clear H0.
+  exists lc1'. split; auto.
+ 
+Case "dbBlocks_cons".
+  inversion d; subst.
+  apply H with (B1:=block_intro l0 ps (cs++cs') tmn)(als0:=als)(Mem:=Mem0) 
+               (B1':=B')(als':=als3)(Mem':=Mem3)(lc3:=lc5) in H3; auto.
+  clear H.
+  destruct H3 as [lc5' [HdbBlock Heq5]].
+  apply H0 with (als'0:=als')(als:=als3)(Mem:=Mem3)(Mem'0:=Mem')(lc3:=lc2)(B1:=B')(B1'0:=B1') in Heq5; auto.
+  clear H0.
+  destruct Heq5 as [lc2' [HdbBlocks Heq2]].
+  exists lc2'. split; eauto.
+
+Case "dbFdef_func".
+  rewrite e in H1. inversion H1; subst. clear H1.
+  assert (J:=@eqAL_initLocals la0 lp TD lc gl lc1' H2).
+  apply H with (B1:=block_intro l1 ps1 cs1 tmn1)(als:=nil)(Mem:=Mem0)(lc3:=lc1)
+               (B1':=block_intro l2 ps2 (cs21++cs22) (insn_return rid rt Result))(als':=als1)(Mem':=Mem1) in J; auto.
+  clear H. destruct J as [lc2' [HdbBlocks Heq2]].
+  rewrite eqAL_params2GVs with (lc':=lc1') in HdbBlocks; eauto.
+  apply H0 in Heq2. clear H0.
+  destruct Heq2 as [lc3' [Hsubblocks Heq3]].
+  apply dbCmds_eqEnv with (lc1':=lc3') in d1; auto.
+  destruct d1 as [lc4' [HdbCmds Heq4]].
+  exists lc4'. split; eauto.
+    eapply dbFdef_func; eauto.
+      erewrite eqAL_lookupExFdefViaGV; eauto using eqAL_sym.
+
+Case "dbFdef_proc".
+  rewrite e in H1. inversion H1; subst. clear H1.
+  assert (J:=@eqAL_initLocals la0 lp TD lc gl lc1' H2).
+  apply H with (B1:=block_intro l1 ps1 cs1 tmn1)(als:=nil)(Mem:=Mem0)(lc3:=lc1)
+               (B1':=block_intro l2 ps2 (cs21++cs22) (insn_return_void rid))(als':=als1)(Mem':=Mem1) in J; auto.
+  clear H. destruct J as [lc2' [HdbBlocks Heq2]].
+  rewrite eqAL_params2GVs with (lc':=lc1') in HdbBlocks; eauto.
+  apply H0 in Heq2. clear H0.
+  destruct Heq2 as [lc3' [Hsubblocks Heq3]].
+  apply dbCmds_eqEnv with (lc1':=lc3') in d1; auto.
+  destruct d1 as [lc4' [HdbCmds Heq4]].
+  exists lc4'. split; eauto.
+    eapply dbFdef_proc; eauto.
+      erewrite eqAL_lookupExFdefViaGV; eauto using eqAL_sym.
+Qed.
+
+Lemma dbCall_eqEnv : forall S TD Ps fs gl lc1 Mem0 call0 lc2 Mem' tr lc1',
+  dbCall S TD Ps fs gl lc1 Mem0 call0 lc2 Mem' tr ->
+  eqAL _ lc1 lc1' ->
+  exists lc2',
+    dbCall S TD Ps fs gl lc1' Mem0 call0 lc2' Mem' tr /\
+    eqAL _ lc2 lc2'.
+Proof.
+  intros.
+  destruct db_eqEnv as [J _].
+  unfold dbCall_eqEnv_prop in J. eauto.
+Qed.
+
+Lemma dbSubblock_eqEnv : forall S TD Ps fs gl lc1 als Mem cs lc2 als' Mem' tr lc1',
+  dbSubblock S TD Ps fs gl lc1 als Mem cs lc2 als' Mem' tr ->
+  eqAL _ lc1 lc1' ->
+  exists lc2',
+    dbSubblock S TD Ps fs gl lc1' als Mem cs lc2' als' Mem' tr /\
+    eqAL _ lc2 lc2'.
+Proof.
+  intros.
+  destruct db_eqEnv as [_ [J _]].
+  unfold dbSubblock_eqEnv_prop in J. eauto.
+Qed.
+
+Lemma dbSubblocks_eqEnv : forall S TD Ps fs gl lc1 als Mem cs lc2 als' Mem' tr lc1',
+  dbSubblocks S TD Ps fs gl lc1 als Mem cs lc2 als' Mem' tr ->
+  eqAL _ lc1 lc1' ->
+  exists lc2',
+    dbSubblocks S TD Ps fs gl lc1' als Mem cs lc2' als' Mem' tr /\
+    eqAL _ lc2 lc2'.
+Proof.
+  intros.
+  destruct db_eqEnv as [_ [_ [J _]]].
+  unfold dbSubblocks_eqEnv_prop in J. eauto.
+Qed.
+
+Lemma dbBlock_eqEnv : forall S TD Ps fs gl F arg tr B1 lc1 als Mem B1' lc2 als' Mem' lc1',
+  dbBlock S TD Ps fs gl F arg 
+    (mkState (mkEC B1 lc1 als) Mem) 
+    (mkState (mkEC B1' lc2 als') Mem') 
+    tr ->
+  eqAL _ lc1 lc1' ->
+  exists lc2',
+    dbBlock S TD Ps fs gl F arg 
+     (mkState (mkEC B1 lc1' als) Mem) 
+     (mkState (mkEC B1' lc2' als') Mem') 
+     tr /\
+    eqAL _ lc2 lc2'.
+Proof.
+  intros.
+  destruct db_eqEnv as [_ [_ [_ [J _]]]].
+  unfold dbBlock_eqEnv_prop in J. eauto.
+Qed.
+
+Lemma dbBlocks_eqEnv : forall S TD Ps fs gl F lp tr B1 lc1 als Mem B1' lc2 als' Mem' lc1',
+  dbBlocks S TD Ps fs gl F lp
+    (mkState (mkEC B1 lc1 als) Mem)
+    (mkState (mkEC B1' lc2 als') Mem')
+    tr ->
+  eqAL _ lc1 lc1' ->
+  exists lc2',
+    dbBlocks S TD Ps fs gl F lp 
+     (mkState (mkEC B1 lc1' als) Mem) 
+     (mkState (mkEC B1' lc2' als') Mem') 
+     tr /\
+    eqAL _ lc2 lc2'.
+Proof.
+  intros.
+  destruct db_eqEnv as [_ [_ [_ [_ [J _]]]]].
+  unfold dbBlocks_eqEnv_prop in J. eauto.
+Qed.
+
+Lemma dbFdef_eqEnv : forall fv fid rt lp S TD Ps lc1 gl fs Mem lc2 als' Mem' B' Rid oResult tr la lb lc1',
+  dbFdef fv rt lp S TD Ps lc1 gl fs Mem lc2 als' Mem' B' Rid oResult tr ->
+  lookupFdefViaGV TD Ps gl lc1 fs fv = Some (fdef_intro (fheader_intro rt fid la) lb) ->
+  eqAL _ lc1 lc1' ->
+  exists lc2',
+    dbFdef fv rt lp S TD Ps lc1' gl fs Mem lc2' als' Mem' B' Rid oResult tr /\
+    eqAL _ lc2 lc2'.
+Proof.
+  intros.
+  destruct db_eqEnv as [_ [_ [_ [_ [_ J]]]]].
+  unfold dbFdef_eqEnv_prop in J. eauto.
+Qed.
+
+(* subAL *)
+
+Definition subAL X lc1 lc2 := 
+  forall i, i `in` dom lc1 -> lookupAL X lc1 i = lookupAL X lc2 i.
+
+Notation "lc1 <<<= lc2" := (subAL _ lc1 lc2) (at level 70, no associativity).
+
+Lemma lookupAL_app1 : forall X (lc1:list (atom*X)) lc2 i,
+  i `in` dom lc1 ->
+  lookupAL X lc1 i = lookupAL X (lc1++lc2) i.
+Proof.
+  induction lc1; intros lc2 i Hi_in_lc1.
+    fsetdec.
+    destruct a as (id, elt); simpl in *.
+    destruct (@eq_dec atom (EqDec_eq_of_EqDec atom EqDec_atom) i id); auto.
+      apply IHlc1. fsetdec.
+Qed.    
+
+Lemma lookupAL_app2 : forall X lc1 (lc2:list (atom*X)) i,
+  i `notin` dom lc1 ->
+  lookupAL X lc2 i = lookupAL X (lc1++lc2) i.
+Proof.
+  induction lc1; intros lc2 i Hi_notin_lc1; auto.
+    destruct a as (id, elt); simpl in *.
+    destruct (@eq_dec atom (EqDec_eq_of_EqDec atom EqDec_atom) i id); subst; eauto.
+      fsetdec.
+Qed.    
+
+Lemma subAL_app1 : forall X (lc1:list (atom*X)) lc2 lc,
+  lc1 <<<= lc ->
+  lc2 <<<= lc ->
+  lc1 ++ lc2 <<<= lc.
+Proof.
+  intros X lc1 lc2 lc Hlc1_sub_lc Hlc2_sub_lc.
+  intros i i_in_lc12.
+  simpl_env in i_in_lc12.
+  apply in_dom_app_inv in i_in_lc12.
+  assert (i `in`  dom lc1 \/ i `notin` dom lc1) as i_in_lc1_dec. fsetdec.
+  destruct i_in_lc1_dec as [i_in_lc1 | i_notin_lc1].
+    rewrite <- Hlc1_sub_lc; auto.
+    rewrite <- lookupAL_app1; auto.
+
+    destruct i_in_lc12 as [i_in_lc1 | i_in_lc2].
+      fsetdec.
+      rewrite <- lookupAL_app2; auto.
+Qed.
+
+Lemma lookupALs_tail : forall X l2b l2b' l0,
+  l0 `notin` dom l2b ->
+  lookupAL X (l2b++l2b') l0 = lookupAL _ l2b' l0.
+Proof.
+  intros.
+  induction l2b; auto.
+    destruct a. simpl in *.
+    destruct (@eq_dec atom (@EqDec_eq_of_EqDec atom EqDec_atom) l0 a); subst; auto.
+      fsetdec.
+Qed.
+
+Lemma subAL_app2 : forall X (lc1:list (atom*X)) lc2 lc,
+  lc1 <<<= lc ->
+  disjoint lc1 lc2 ->
+  ~ lc2 <<<= lc ->
+  ~ lc1 ++ lc2 <<<= lc.
+Proof.
+  intros X lc1 lc2 lc Hlc1_sub_lc Hdisj Hlc2_nsub_lc Hlc12_sub_lc.
+  apply Hlc2_nsub_lc.
+  intros i i_in_lc2.
+    assert (i `notin` dom lc1) as i_notin_lc1. solve_uniq.
+    assert (i `in` dom (lc1++lc2)) as i_in_lc12. simpl_env. fsetdec.
+    apply Hlc12_sub_lc in i_in_lc12.
+    erewrite lookupALs_tail in i_in_lc12; eauto.
+Qed.
+    
+(* subAL *)
+
+Lemma getOperandValue_subAL : forall lc1 gl lc2 v TD gv,
+  subAL _ lc1 lc2 ->
+  getOperandValue TD v lc1 gl = Some gv ->
+  getOperandValue TD v lc1 gl = getOperandValue TD v lc2 gl.
+Proof.
+  intros lc1 gl lc2 v TD gv Hnon_none HeqAL.
+  unfold getOperandValue in *.
+  destruct v; auto.
+    apply lookupAL_Some_indom in HeqAL. eauto.
+Qed.
+
+Lemma subAL_updateAddAL : forall X lc1 lc2 id0 gv0,
+  subAL X lc1 lc2 ->
+  subAL _ (updateAddAL _ lc1 id0 gv0) (updateAddAL _ lc2 id0 gv0).
+Proof.
+  unfold subAL. 
+  intros.
+  rewrite updateAddAL_dom_eq in H0.
+  destruct (id0==i0); subst.
+    rewrite lookupAL_updateAddAL_eq; auto.
+    rewrite lookupAL_updateAddAL_eq; auto.
+
+    assert (i0 `in` dom lc1) as Hi0_in_lc1. fsetdec.
+    assert (J:=H i0 Hi0_in_lc1).
+    erewrite <- lookupAL_updateAddAL_neq; eauto.
+    erewrite <- lookupAL_updateAddAL_neq; eauto.
+Qed.
+
+Lemma subAL_callUpdateLocals : forall TD noret0 rid rt oResult lc1 lc2 gl lc1' lc2',
+  subAL _ lc1 lc1' ->
+  subAL _ lc2 lc2' ->
+  subAL _ (callUpdateLocals TD noret0 rid rt oResult lc1 lc2 gl)
+         (callUpdateLocals TD noret0 rid rt oResult lc1' lc2' gl).
+Proof.
+  intros TD noret0 rid rt oResult lc1 lc2 gl lc1' lc2' H1 H2.
+    unfold callUpdateLocals.
+    destruct noret0; auto.
+      destruct (rt=t=typ_void); auto.
+        destruct oResult; simpl; auto.
+          destruct v; simpl.
+            remember (lookupAL _ lc2 i0) as Lookup.
+            destruct Lookup as [gr | _].
+              rewrite H2 in HeqLookup; eauto using lookupAL_Some_indom.
+              rewrite <- HeqLookup. apply subAL_updateAddAL; auto.
+
+              (* We should prove that if oResult is Some, i0 in lc2. *)
+              admit.
+
+          destruct (const2GV TD gl c); auto using subAL_updateAddAL.
+Qed.
+
+Lemma subAL_refl : forall X lc,
+  subAL X lc lc.
+Proof. unfold subAL. auto. Qed.
+
+Lemma subAL_getIncomingValuesForBlockFromPHINodes : forall TD ps B gl lc lc',
+  subAL _ lc lc' ->
+  getIncomingValuesForBlockFromPHINodes TD ps B gl lc =
+  getIncomingValuesForBlockFromPHINodes TD ps B gl lc'.
+Proof.
+  induction ps; intros; simpl; auto.
+    destruct a; auto.
+    destruct (getValueViaBlockFromValuels l0 B); auto.
+    destruct v; erewrite IHps; eauto.
+      (* We should redefine getIncomingValuesForBlockFromPHINodes to be partial. 
+         If we cannot find any incoming value, we should return None. *)
+      assert (i1 `in` dom lc) as J. admit. 
+      rewrite H; auto.
+Qed.
+
+Lemma subAL_updateValuesForNewBlock : forall vs lc lc',
+  subAL _ lc lc' ->
+  subAL _ (updateValuesForNewBlock vs lc) (updateValuesForNewBlock vs lc').
+Proof.
+  induction vs; intros; simpl; auto.
+    destruct a.
+    destruct o; auto using subAL_updateAddAL.
+Qed.
+
+Lemma subAL_switchToNewBasicBlock : forall TD B1 B2 gl lc lc',
+  subAL _ lc lc' ->
+  subAL _ (switchToNewBasicBlock TD B1 B2 gl lc) (switchToNewBasicBlock TD B1 B2 gl lc').
+Proof.
+  intros.
+  unfold switchToNewBasicBlock.
+  erewrite subAL_getIncomingValuesForBlockFromPHINodes; eauto.
+  apply subAL_updateValuesForNewBlock; auto.
+Qed.
+
+Lemma subAL_exCallUpdateLocals : forall noret0 rid rt oResult lc lc',
+  subAL _ lc lc' ->
+  subAL _ (exCallUpdateLocals noret0 rid rt oResult lc)
+         (exCallUpdateLocals noret0 rid rt oResult lc').
+Proof.
+  intros noret0 rid rt oResult lc lc' H1.
+    unfold exCallUpdateLocals.
+    destruct noret0; auto.
+      destruct (rt=t=typ_void); auto.
+        destruct oResult; simpl; auto using subAL_updateAddAL.
+Qed.
+
+Lemma subAL_lookupExFdecViaGV : forall gl TD Ps lc lc' fs fv gv,
+  subAL _ lc lc' ->
+  lookupExFdecViaGV TD Ps gl lc fs fv = Some gv ->
+  lookupExFdecViaGV TD Ps gl lc fs fv = lookupExFdecViaGV TD Ps gl lc' fs fv.
+Proof.
+  intros.
+  unfold lookupExFdecViaGV in *.
+  assert (exists gv, getOperandValue TD fv lc gl = Some gv) as J.
+    destruct (getOperandValue TD fv lc gl); eauto.
+      inversion H0.
+  destruct J as [gv' J].
+  erewrite getOperandValue_subAL; eauto.
+Qed.
+
+Lemma subAL_lookupExFdefViaGV : forall gl TD Ps lc lc' fs fv gv,
+  subAL _ lc lc' ->
+  lookupFdefViaGV TD Ps gl lc fs fv = Some gv ->
+  lookupFdefViaGV TD Ps gl lc fs fv = lookupFdefViaGV TD Ps gl lc' fs fv.
+Proof.
+  intros.
+  unfold lookupFdefViaGV in *.
+  assert (exists gv, getOperandValue TD fv lc gl = Some gv) as J.
+    destruct (getOperandValue TD fv lc gl); eauto.
+      inversion H0.
+  destruct J as [gv' J].
+  erewrite getOperandValue_subAL; eauto.
+Qed.
+
+Lemma subAL_params2OpGVs : forall lp TD lc gl lc',
+  subAL _ lc lc' ->
+  params2OpGVs TD lp lc gl = params2OpGVs TD lp lc' gl.
+Proof.
+  induction lp; intros; simpl; auto.
+    destruct a.
+    destruct v; simpl.
+      (* We should redefine params2OpGVs to be partial. 
+         If we cannot find any param value, we should return None. *)
+      assert (i0 `in` dom lc) as J. admit. 
+      rewrite H; auto. erewrite IHlp; eauto.
+      erewrite IHlp; eauto.
+Qed.
+
+Lemma subAL_params2GVs : forall lp TD lc gl lc',
+  subAL _ lc lc' ->
+  params2GVs TD lp lc gl = params2GVs TD lp lc' gl.
+Proof.
+  induction lp; intros; simpl; auto.
+    destruct a.
+    unfold params2GVs.
+    erewrite subAL_params2OpGVs; eauto.
+Qed.
+
+Lemma subAL_initLocals : forall la lp TD lc gl lc',
+  subAL _ lc lc' ->
+  subAL _ (initLocals la (params2GVs TD lp lc gl)) (initLocals la (params2GVs TD lp lc' gl)).
+Proof.
+  intros. erewrite subAL_params2GVs; eauto using subAL_refl.
+  (* This lemma will be broken if we fix subAL_params2GVs 
+     The problem is that the Fdef rule should check that params2GVs lp = Some ... *)
+Qed.
+
+Lemma BOP_subAL : forall lc1 gl lc2 bop0 sz0 v1 v2 TD gv,
+  subAL _ lc1 lc2 ->
+  BOP TD lc1 gl bop0 sz0 v1 v2 = Some gv ->
+  BOP TD lc1 gl bop0 sz0 v1 v2 = BOP TD lc2 gl bop0 sz0 v1 v2.
+Proof.
+  intros lc1 gl lc2 bop0 sz0 v1 v2 TD gv HsubEnv Hsome.
+  apply BOP_inversion in Hsome.
+  destruct Hsome as [gv1 [gv2 [Hsome1 [Hsome2 _]]]].
+  unfold BOP in *.
+  erewrite getOperandValue_subAL with (lc2:=lc2)(v:=v1); eauto.
+  erewrite getOperandValue_subAL with (lc2:=lc2)(v:=v2); eauto.
+Qed.
+
+Lemma FBOP_subAL : forall lc1 gl lc2 fbop0 fp0 v1 v2 TD gv,
+  subAL _ lc1 lc2 ->
+  FBOP TD lc1 gl fbop0 fp0 v1 v2 = Some gv ->
+  FBOP TD lc1 gl fbop0 fp0 v1 v2 = FBOP TD lc2 gl fbop0 fp0 v1 v2.
+Proof.
+  intros lc1 gl lc2 fbop0 fp0 v1 v2 TD gv HsubEnv Hsome.
+  apply FBOP_inversion in Hsome.
+  destruct Hsome as [gv1 [gv2 [Hsome1 [Hsome2 _]]]].
+  unfold FBOP in *.
+  rewrite getOperandValue_subAL with (lc2:=lc2)(v:=v1)(gv:=gv1); auto.
+  rewrite getOperandValue_subAL with (lc2:=lc2)(v:=v2)(gv:=gv2); auto.
+Qed.
+
+Lemma getOperandPtr_subAL : forall lc1 gl lc2 v TD gv,
+  subAL _ lc1 lc2 ->
+  getOperandPtr TD v lc1 gl = Some gv ->
+  getOperandPtr TD v lc1 gl = getOperandPtr TD v lc2 gl.
+Proof.
+  intros lc1 gl lc2 v TD gv HsubEnv Hsome.
+  apply getOperandPtr_inversion in Hsome.
+  destruct Hsome as [gv0 [Hsome _]].
+  unfold getOperandPtr in *.
+  erewrite getOperandValue_subAL; eauto.
+Qed.
+
+Lemma getOperandInt_subAL : forall lc1 gl lc2 sz v TD gv,
+  subAL _ lc1 lc2 ->
+  getOperandInt TD sz v lc1 gl = Some gv ->
+  getOperandInt TD sz v lc1 gl = getOperandInt TD sz v lc2 gl.
+Proof.
+  intros lc1 gl lc2 sz0 v TD gv HsubAL Hsome.
+  apply getOperandInt_inversion in Hsome.
+  destruct Hsome as [gv0 [Hsome _]].
+  unfold getOperandInt in *.
+  erewrite getOperandValue_subAL; eauto.
+Qed.
+
+Lemma getOperandPtrInBits_subAL : forall lc1 gl lc2 sz v TD gv,
+  subAL _ lc1 lc2 ->
+  getOperandValue TD v lc1 gl = Some gv ->
+  getOperandPtrInBits TD sz v lc1 gl = getOperandPtrInBits TD sz v lc2 gl.
+Proof.
+  intros lc1 gl lc2 sz0 v TD gv HsubAL Hsome.
+  unfold getOperandPtrInBits in *.
+  erewrite getOperandValue_subAL; eauto.
+Qed.
+
+Lemma CAST_subAL : forall lc1 gl lc2 op t1 v1 t2 TD gv,
+  subAL _ lc1 lc2 ->
+  CAST TD lc1 gl op t1 v1 t2 = Some gv ->
+  CAST TD lc1 gl op t1 v1 t2 = CAST TD lc2 gl op t1 v1 t2.
+Proof.
+  intros lc1 gl lc2 op t1 v1 t2 TD gv HsubAL Hsome.
+  apply CAST_inversion in Hsome.
+  destruct Hsome as [gv1 [Hsome _]].
+  unfold CAST in *.
+  rewrite getOperandValue_subAL with (lc2:=lc2)(v:=v1)(gv:=gv1); auto.
+Qed.
+
+Lemma TRUNC_subAL : forall lc1 gl lc2 op t1 v1 t2 TD gv,
+  subAL _ lc1 lc2 ->
+  TRUNC TD lc1 gl op t1 v1 t2 = Some gv ->
+  TRUNC TD lc1 gl op t1 v1 t2 = TRUNC TD lc2 gl op t1 v1 t2.
+Proof.
+  intros lc1 gl lc2 op t1 v1 t2 TD gv HsubAL Hsome.
+  apply TRUNC_inversion in Hsome.
+  destruct Hsome as [gv1 [Hsome _]].
+  unfold TRUNC in *.
+  rewrite getOperandValue_subAL with (lc2:=lc2)(v:=v1)(gv:=gv1); auto.
+Qed.
+
+Lemma EXT_subAL : forall lc1 gl lc2 op t1 v1 t2 TD gv,
+  subAL _ lc1 lc2 ->
+  EXT TD lc1 gl op t1 v1 t2 = Some gv ->
+  EXT TD lc1 gl op t1 v1 t2 = EXT TD lc2 gl op t1 v1 t2.
+Proof.
+  intros lc1 gl lc2 op t1 v1 t2 TD gv HsubAL Hsome.
+  apply EXT_inversion in Hsome.
+  destruct Hsome as [gv1 [Hsome _]].
+  unfold EXT in *.
+  rewrite getOperandValue_subAL with (lc2:=lc2)(v:=v1)(gv:=gv1); auto.
+Qed.
+
+Lemma ICMP_subAL : forall lc1 gl lc2 cond t v1 v2 TD gv,
+  subAL _ lc1 lc2 ->
+  ICMP TD lc1 gl cond t v1 v2 = Some gv ->
+  ICMP TD lc1 gl cond t v1 v2 = ICMP TD lc2 gl cond t v1 v2.
+Proof.
+  intros lc1 gl lc2 cond0 t v1 v2 TD gv HsubAL Hsome.
+  apply ICMP_inversion in Hsome.
+  destruct Hsome as [gv1 [gv2 [Hsome1 [Hsome2 _]]]].
+  unfold ICMP in *.
+  rewrite getOperandValue_subAL with (lc2:=lc2)(v:=v1)(gv:=gv1); auto.
+  rewrite getOperandValue_subAL with (lc2:=lc2)(v:=v2)(gv:=gv2); auto.
+Qed.
+
+Lemma FCMP_subAL : forall lc1 gl lc2 cond fp v1 v2 TD gv,
+  subAL _ lc1 lc2 ->
+  FCMP TD lc1 gl cond fp v1 v2 = Some gv ->
+  FCMP TD lc1 gl cond fp v1 v2 = FCMP TD lc2 gl cond fp v1 v2.
+Proof.
+  intros lc1 gl lc2 cond0 fp v1 v2 TD gv HsubAL Hsome.
+  apply FCMP_inversion in Hsome.
+  destruct Hsome as [gv1 [gv2 [Hsome1 [Hsome2 _]]]].
+  unfold FCMP in *.
+  rewrite getOperandValue_subAL with (lc2:=lc2)(v:=v1)(gv:=gv1); auto.
+  rewrite getOperandValue_subAL with (lc2:=lc2)(v:=v2)(gv:=gv2); auto.
+Qed.
+
+Lemma intValues2Nats_subAL : forall l0 lc1 gl lc2 TD zs,
+  subAL _ lc1 lc2 ->
+  intValues2Nats TD l0 lc1 gl = Some zs ->
+  intValues2Nats TD l0 lc1 gl = intValues2Nats TD l0 lc2 gl.
+Proof.
+  induction l0; intros lc1 gl lc2 TD zs HsubAL Hsome; simpl in *; auto.
+    assert (exists gv, getOperandValue TD v lc1 gl = Some gv) as J.
+      destruct (getOperandValue TD v lc1 gl); eauto.
+        inversion Hsome.
+    destruct J as [gv J].
+    erewrite getOperandValue_subAL with (lc2:=lc2)(v:=v); eauto.
+      rewrite J in Hsome.
+      destruct (GV2int TD Size.ThirtyTwo gv); try solve [inversion Hsome].
+      assert (exists zs', intValues2Nats TD l0 lc1 gl = Some zs') as J'.
+        destruct (intValues2Nats TD l0 lc1 gl); eauto.
+      destruct J' as [gv' J'].
+      erewrite IHl0; eauto.
+Qed.
+
+Lemma values2GVs_subAL : forall l0 lc1 gl lc2 TD gvs,
+  subAL _ lc1 lc2 ->
+  values2GVs TD l0 lc1 gl = Some gvs ->
+  values2GVs TD l0 lc1 gl = values2GVs TD l0 lc2 gl.
+Proof.
+  induction l0; intros lc1 gl lc2 TD gvs HsubAL Hsome; simpl in *; auto.
+    assert (exists gv, getOperandValue TD v lc1 gl = Some gv) as J.
+      destruct (getOperandValue TD v lc1 gl); eauto.
+        inversion Hsome.
+    destruct J as [gv J].
+    erewrite getOperandValue_subAL with (lc2:=lc2)(v:=v); eauto.
+      rewrite J in Hsome.
+      assert (exists gvs', values2GVs TD l0 lc1 gl = Some gvs') as J'.
+        destruct (values2GVs TD l0 lc1 gl); eauto.
+      destruct J' as [gvs' J'].
+      erewrite IHl0; eauto.
+Qed.
+
+(* subEnv *)
+
+Lemma dbCmd_subEnv : forall TD c lc1 als1 gl Mem1 lc2 als2 Mem2 tr lc1',
+  dbCmd TD gl lc1 als1 Mem1 c lc2 als2 Mem2 tr ->
+  subAL _ lc1 lc1' ->
+  exists lc2', 
+    dbCmd TD gl lc1' als1 Mem1 c lc2' als2 Mem2 tr /\
+    subAL _ lc2 lc2'.
+Proof.
+  intros TD c lc1 als1 gl Mem1 lc2 als2 Mem2 tr lc1' HdbCmd HsubEnv.
+  (dbCmd_cases (inversion HdbCmd) Case); subst.
+Case "dbBop".
+  assert (HupdateEnv:=HsubEnv).
+  exists (updateAddAL _ lc1' id0 gv3).
+  erewrite BOP_subAL with (lc2:=lc1') in H; eauto.
+  split; eauto using subAL_updateAddAL.
+
+Case "dbFBop".
+  assert (HupdateEnv:=HsubEnv).
+  exists (updateAddAL _ lc1' id0 gv3).
+  erewrite FBOP_subAL with (lc2:=lc1') in H; eauto.
+  split; eauto using subAL_updateAddAL.
+
+Case "dbExtractValue".
+  assert (HupdateEnv:=HsubEnv).
+  exists (updateAddAL _ lc1' id0 gv').
+  erewrite getOperandValue_subAL with (lc2:=lc1') in H; eauto. 
+  split; eauto using subAL_updateAddAL.
+  
+Case "dbInsertValue".
+  assert (HupdateEnv:=HsubEnv).
+  exists (updateAddAL _ lc1' id0 gv'').
+  erewrite getOperandValue_subAL with (lc2:=lc1') in H; eauto. 
+  erewrite getOperandValue_subAL with (lc2:=lc1') in H0; eauto. 
+  split; eauto using subAL_updateAddAL.
+
+Case "dbMalloc".
+  assert (HupdateEnv:=HsubEnv).
+  exists (updateAddAL _ lc1' id0 (blk2GV TD mb)).
+  erewrite getOperandValue_subAL with (lc2:=lc1') in H0; eauto. 
+  split; eauto using subAL_updateAddAL.
+
+Case "dbFree".
+  exists lc1'.
+  erewrite getOperandValue_subAL with (lc2:=lc1') in H; eauto. 
+
+Case "dbAlloca".
+  assert (HupdateEnv:=HsubEnv).
+  exists (updateAddAL _ lc1' id0 (blk2GV TD mb)).
+  erewrite getOperandValue_subAL with (lc2:=lc1') in H0; eauto. 
+  split; eauto using subAL_updateAddAL.
+
+Case "dbLoad".
+  assert (HupdateEnv:=HsubEnv).
+  exists (updateAddAL _ lc1' id0 gv).
+  erewrite getOperandValue_subAL with (lc2:=lc1') in H; eauto. 
+  split; eauto using subAL_updateAddAL.
+
+Case "dbStore".
+  exists lc1'.
+  erewrite getOperandValue_subAL with (lc2:=lc1') in H; eauto. 
+  erewrite getOperandValue_subAL with (lc2:=lc1') in H0; eauto. 
+
+Case "dbGEP".
+  assert (HupdateEnv:=HsubEnv).
+  exists (updateAddAL _ lc1' id0 mp').
+  erewrite getOperandValue_subAL with (lc2:=lc1') in H; eauto. 
+  erewrite values2GVs_subAL with (lc2:=lc1') in H0; eauto. 
+(* rewrite GEP_eqAL with (lc2:=lc1') in H0; auto. *)
+  split; eauto using subAL_updateAddAL.
+
+Case "dbTrunc".
+  assert (HupdateEnv:=HsubEnv).
+  exists (updateAddAL _ lc1' id0 gv2).
+  erewrite TRUNC_subAL with (lc2:=lc1') in H; eauto.
+  split; eauto using subAL_updateAddAL.
+
+Case "dbExt".
+  assert (HupdateEnv:=HsubEnv).
+  exists (updateAddAL _ lc1' id0 gv2).
+  erewrite EXT_subAL with (lc2:=lc1') in H; eauto.
+  split; eauto using subAL_updateAddAL.
+
+Case "dbCast".
+  assert (HupdateEnv:=HsubEnv).
+  exists (updateAddAL _ lc1' id0 gv2).
+  erewrite CAST_subAL with (lc2:=lc1') in H; eauto.
+  split; eauto using subAL_updateAddAL.
+
+Case "dbIcmp".
+  assert (HupdateEnv:=HsubEnv).
+  exists (updateAddAL _ lc1' id0 gv3).
+  erewrite ICMP_subAL with (lc2:=lc1') in H; eauto.
+  split; eauto using subAL_updateAddAL.
+
+Case "dbFcmp".
+  assert (HupdateEnv:=HsubEnv).
+  exists (updateAddAL _ lc1' id0 gv3).
+  erewrite FCMP_subAL with (lc2:=lc1') in H; eauto.
+  split; eauto using subAL_updateAddAL.
+
+Case "dbSelect".
+  erewrite getOperandValue_subAL with (lc2:=lc1') in H; eauto. 
+  erewrite getOperandValue_subAL with (lc2:=lc1') in H0; eauto. 
+  erewrite getOperandValue_subAL with (lc2:=lc1') in H1; eauto. 
+  assert (HupdateEnv:=HsubEnv).
+  exists (if isGVZero TD cond0 then updateAddAL _ lc1' id0 gv2 else updateAddAL _ lc1' id0 gv1).
+  split; auto.
+    destruct (isGVZero TD cond0); auto using subAL_updateAddAL.
+Qed.
+
+Lemma dbCmds_subEnv : forall TD cs lc1 als1 gl Mem1 lc2 als2 Mem2 tr lc1',
+  dbCmds TD gl lc1 als1 Mem1 cs lc2 als2 Mem2 tr ->
+  subAL _ lc1 lc1' ->
+  exists lc2', 
+    dbCmds TD gl lc1' als1 Mem1 cs lc2' als2 Mem2 tr /\
+    subAL _ lc2 lc2'.
+Proof.
+  intros TD cs lc1 als1 gl Mem1 lc2 als2 Mem2 tr lc1' HdbCmds HsubEnv.
+  generalize dependent lc1'.
+  induction HdbCmds; intros.
+    exists lc1'. split; auto.
+
+    apply dbCmd_subEnv with (lc1':=lc1') in H; auto.
+    destruct H as [lc2' [HdbCmd HsubEnv']].
+    apply IHHdbCmds in HsubEnv'; auto.
+    destruct HsubEnv' as [lc3' [HdbCmds' HsubEnv'']].
+    exists lc3'.
+    split; eauto.
+Qed.
+
+Lemma dbTerminator_subEnv : forall TD F gl lc1 tmn lc2 tr lc1' B B',
+  dbTerminator TD F gl B lc1 tmn B' lc2 tr ->
+  subAL _ lc1 lc1' ->
+  exists lc2',
+    dbTerminator TD F gl B lc1' tmn B' lc2' tr /\
+    subAL _ lc2 lc2'.
+Proof.
+  intros TD F gl lc1 tmn lc2 tr lc1' B B' HdbTerminator HsubAL.
+  inversion HdbTerminator; subst.
+    exists (switchToNewBasicBlock TD (block_intro l' ps' sbs' tmn') B gl lc1').
+    split.
+      apply dbBranch with (c:=c); auto.
+        erewrite <- getOperandValue_subAL; eauto.
+      apply subAL_switchToNewBasicBlock; auto.     
+  
+    exists (switchToNewBasicBlock TD (block_intro l' ps' sbs' tmn') B gl lc1').
+    split.
+      apply dbBranch_uncond; auto.
+      apply subAL_switchToNewBasicBlock; auto.
+Qed.     
+
+Definition dbCall_subEnv_prop S TD Ps fs gl lc1 Mem0 call0 lc2 Mem' tr
+  (db:dbCall S TD Ps fs gl lc1 Mem0 call0 lc2 Mem' tr) := 
+  forall lc1',
+  subAL _ lc1 lc1' ->
+  exists lc2',
+    dbCall S TD Ps fs gl lc1' Mem0 call0 lc2' Mem' tr /\
+    subAL _ lc2 lc2'.
+Definition dbSubblock_subEnv_prop S TD Ps fs gl lc1 als Mem cs lc2 als' Mem' tr
+  (db:dbSubblock S TD Ps fs gl lc1 als Mem cs lc2 als' Mem' tr) :=
+  forall lc1',
+  subAL _ lc1 lc1' ->
+  exists lc2',
+    dbSubblock S TD Ps fs gl lc1' als Mem cs lc2' als' Mem' tr /\
+    subAL _ lc2 lc2'.
+Definition dbSubblocks_subEnv_prop S TD Ps fs gl lc1 als Mem cs lc2 als' Mem' tr
+  (db:dbSubblocks S TD Ps fs gl lc1 als Mem cs lc2 als' Mem' tr) :=
+  forall lc1',
+  subAL _ lc1 lc1' ->
+  exists lc2',
+    dbSubblocks S TD Ps fs gl lc1' als Mem cs lc2' als' Mem' tr /\
+    subAL _ lc2 lc2'.
+Definition dbBlock_subEnv_prop S TD Ps fs gl F arg state1 state2 tr
+  (db:dbBlock S TD Ps fs gl F arg state1 state2 tr) :=
+  forall B1 lc1 als Mem B1' lc2 als' Mem' lc1',
+  state1 = mkState (mkEC B1 lc1 als) Mem ->
+  state2 = mkState (mkEC B1' lc2 als') Mem' ->
+  subAL _ lc1 lc1' ->
+  exists lc2',
+    dbBlock S TD Ps fs gl F arg 
+     (mkState (mkEC B1 lc1' als) Mem) 
+     (mkState (mkEC B1' lc2' als') Mem') 
+     tr /\
+    subAL _ lc2 lc2'.
+Definition dbBlocks_subEnv_prop S TD Ps fs gl F lp state1 state2 tr
+  (db:dbBlocks S TD Ps fs gl F lp state1 state2 tr) :=
+  forall B1 lc1 als Mem B1' lc2 als' Mem' lc1',
+  state1 = mkState (mkEC B1 lc1 als) Mem ->
+  state2 = mkState (mkEC B1' lc2 als') Mem' ->
+  subAL _ lc1 lc1' ->
+  exists lc2',
+    dbBlocks S TD Ps fs gl F lp 
+     (mkState (mkEC B1 lc1' als) Mem) 
+     (mkState (mkEC B1' lc2' als') Mem') 
+     tr /\
+    subAL _ lc2 lc2'.
+Definition dbFdef_subEnv_prop fv rt lp S TD Ps lc1 gl fs Mem lc2 als' Mem' B' Rid oResult tr
+  (db:dbFdef fv rt lp S TD Ps lc1 gl fs Mem lc2 als' Mem' B' Rid oResult tr) :=
+  forall fid la lb lc1',
+  lookupFdefViaGV TD Ps gl lc1 fs fv = Some (fdef_intro (fheader_intro rt fid la) lb) ->
+  subAL _ lc1 lc1' ->
+  exists lc2',
+    dbFdef fv rt lp S TD Ps lc1' gl fs Mem lc2' als' Mem' B' Rid oResult tr /\
+    subAL _ lc2 lc2'.
+
+Lemma db_subEnv :
+  (forall S TD Ps fs gl lc Mem0 call0 lc' Mem' tr db, 
+     dbCall_subEnv_prop S TD Ps fs gl lc Mem0 call0 lc' Mem' tr db) /\
+  (forall S TD Ps fs gl lc als Mem sb lc' als' Mem' tr db,
+     dbSubblock_subEnv_prop S TD Ps fs gl lc als Mem sb lc' als' Mem' tr db) /\
+  (forall S TD Ps fs gl lc als Mem sbs lc' als' Mem' tr db,
+     dbSubblocks_subEnv_prop S TD Ps fs gl lc als Mem sbs lc' als' Mem' tr db) /\
+  (forall S TD Ps fs gl F arg state1 state2 tr db,
+     dbBlock_subEnv_prop S TD Ps fs gl F arg state1 state2 tr db) /\
+  (forall S TD Ps fs gl F lp state1 state2 tr db,
+     dbBlocks_subEnv_prop S TD Ps fs gl F lp state1 state2 tr db) /\
+  (forall fid rt lp S TD Ps lc gl fs Mem lc' als' Mem' B' Rid oResult tr db,
+     dbFdef_subEnv_prop fid rt lp S TD Ps lc gl fs Mem lc' als' Mem' B' Rid oResult tr db).
+Proof.
+(db_mutind_cases
+  apply db_mutind with
+    (P  := dbCall_subEnv_prop)
+    (P0 := dbSubblock_subEnv_prop)
+    (P1 := dbSubblocks_subEnv_prop)
+    (P2 := dbBlock_subEnv_prop)
+    (P3 := dbBlocks_subEnv_prop)
+    (P4 := dbFdef_subEnv_prop) Case);
+  unfold dbCall_subEnv_prop, 
+         dbSubblock_subEnv_prop, dbSubblocks_subEnv_prop,
+         dbBlock_subEnv_prop, dbBlocks_subEnv_prop,
+         dbFdef_subEnv_prop; intros; subst; auto.
+Case "dbCall_internal".
+  inversion d; subst.
+    apply H with (lc1':=lc1') in H1; auto. clear H.
+    destruct H1 as [lc2' [HdbBlocks HeqEnv]].
+    exists (callUpdateLocals TD noret0 rid rt (Some Result) lc1' lc2' gl).
+    split; eauto using dbCall_internal, subAL_callUpdateLocals.
+
+    apply H with (lc1':=lc1') in H1; auto. clear H.
+    destruct H1 as [lc2' [HdbBlocks HeqEnv]].
+    exists (callUpdateLocals TD noret0 rid rt None lc1' lc2' gl).
+    split; eauto using dbCall_internal, subAL_callUpdateLocals.
+
+Case "dbCall_external".
+  exists (exCallUpdateLocals noret0 rid rt oresult lc1').
+  split; eauto using subAL_exCallUpdateLocals.
+    eapply dbCall_external; eauto.
+      erewrite <- subAL_lookupExFdecViaGV; eauto.
+    rewrite <- subAL_params2GVs with (lc:=lc); auto.
+
+Case "dbSubblock_intro".
+  apply dbCmds_subEnv with (lc1':=lc1') in d; auto.
+  destruct d as [lc2' [HdbCmds HsubEnv2]].
+  apply H in HsubEnv2. clear H.
+  destruct HsubEnv2 as [lc3' [HdbCall HsubEnv3]].
+  exists lc3'.
+  split; eauto.
+
+Case "dbSubblocks_nil".
+  exists lc1'. split; auto.
+ 
+Case "dbSubblocks_cons".
+  apply H in H1. clear H.
+  destruct H1 as [lc2' [HdbSubblock Heq2]].
+  apply H0 in Heq2. clear H0.
+  destruct Heq2 as [lc3' [HdbSubblocks Heq3]].
+  exists lc3'. split; eauto.
+
+Case "dbBlock_intro".
+  inversion H0; subst. clear H0.
+  inversion H1; subst. clear H1.
+  apply H in H2. clear H.
+  destruct H2 as [lc2' [HdbSubblocks Heq2]].
+  apply dbCmds_subEnv with (lc1':=lc2') in d0; auto.
+  destruct d0 as [lc3' [HdbCmds Heq3]].
+  apply dbTerminator_subEnv with (lc1':=lc3') in d1; auto.
+  destruct d1 as [lc5' [HdbTerminator Heq5]].
+  exists lc5'. split; eauto.
+
+Case "dbBlocks_nil".
+  inversion H0; subst. clear H0.
+  exists lc1'. split; auto.
+ 
+Case "dbBlocks_cons".
+  inversion d; subst.
+  apply H with (B1:=block_intro l0 ps (cs++cs') tmn)(als0:=als)(Mem:=Mem0) 
+               (B1':=B')(als':=als3)(Mem':=Mem3)(lc3:=lc5) in H3; auto.
+  clear H.
+  destruct H3 as [lc5' [HdbBlock Heq5]].
+  apply H0 with (als'0:=als')(als:=als3)(Mem:=Mem3)(Mem'0:=Mem')(lc3:=lc2)(B1:=B')(B1'0:=B1') in Heq5; auto.
+  clear H0.
+  destruct Heq5 as [lc2' [HdbBlocks Heq2]].
+  exists lc2'. split; eauto.
+
+Case "dbFdef_func".
+  rewrite e in H1. inversion H1; subst. clear H1.
+  assert (J:=@subAL_initLocals la0 lp TD lc gl lc1' H2).
+  apply H with (B1:=block_intro l1 ps1 cs1 tmn1)(als:=nil)(Mem:=Mem0)(lc3:=lc1)
+               (B1':=block_intro l2 ps2 (cs21++cs22) (insn_return rid rt Result))(als':=als1)(Mem':=Mem1) in J; auto.
+  clear H. destruct J as [lc2' [HdbBlocks Hsub2]].
+  rewrite subAL_params2GVs with (lc':=lc1') in HdbBlocks; eauto.
+  apply H0 in Hsub2. clear H0.
+  destruct Hsub2 as [lc3' [Hsubblocks Hsub3]].
+  apply dbCmds_subEnv with (lc1':=lc3') in d1; auto.
+  destruct d1 as [lc4' [HdbCmds Hsub4]].
+  exists lc4'. split; eauto.
+    eapply dbFdef_func; eauto.
+      erewrite <- subAL_lookupExFdefViaGV; eauto.
+
+Case "dbFdef_proc".
+  rewrite e in H1. inversion H1; subst. clear H1.
+  assert (J:=@subAL_initLocals la0 lp TD lc gl lc1' H2).
+  apply H with (B1:=block_intro l1 ps1 cs1 tmn1)(als:=nil)(Mem:=Mem0)(lc3:=lc1)
+               (B1':=block_intro l2 ps2 (cs21++cs22) (insn_return_void rid))(als':=als1)(Mem':=Mem1) in J; auto.
+  clear H. destruct J as [lc2' [HdbBlocks Hsub2]].
+  rewrite subAL_params2GVs with (lc':=lc1') in HdbBlocks; eauto.
+  apply H0 in Hsub2. clear H0.
+  destruct Hsub2 as [lc3' [Hsubblocks Hsub3]].
+  apply dbCmds_subEnv with (lc1':=lc3') in d1; auto.
+  destruct d1 as [lc4' [HdbCmds Hsub4]].
+  exists lc4'. split; eauto.
+    eapply dbFdef_proc; eauto.
+      erewrite <- subAL_lookupExFdefViaGV; eauto.
+Qed.
+
+Lemma dbCall_subEnv : forall S TD Ps fs gl lc1 Mem0 call0 lc2 Mem' tr lc1',
+  dbCall S TD Ps fs gl lc1 Mem0 call0 lc2 Mem' tr ->
+  subAL _ lc1 lc1' ->
+  exists lc2',
+    dbCall S TD Ps fs gl lc1' Mem0 call0 lc2' Mem' tr /\
+    subAL _ lc2 lc2'.
+Proof.
+  intros.
+  destruct db_subEnv as [J _].
+  unfold dbCall_subEnv_prop in J. eauto.
+Qed.
+
+Lemma dbSubblock_subEnv : forall S TD Ps fs gl lc1 als Mem cs lc2 als' Mem' tr lc1',
+  dbSubblock S TD Ps fs gl lc1 als Mem cs lc2 als' Mem' tr ->
+  subAL _ lc1 lc1' ->
+  exists lc2',
+    dbSubblock S TD Ps fs gl lc1' als Mem cs lc2' als' Mem' tr /\
+    subAL _ lc2 lc2'.
+Proof.
+  intros.
+  destruct db_subEnv as [_ [J _]].
+  unfold dbSubblock_subEnv_prop in J. eauto.
+Qed.
+
+Lemma dbSubblocks_subEnv : forall S TD Ps fs gl lc1 als Mem cs lc2 als' Mem' tr lc1',
+  dbSubblocks S TD Ps fs gl lc1 als Mem cs lc2 als' Mem' tr ->
+  subAL _ lc1 lc1' ->
+  exists lc2',
+    dbSubblocks S TD Ps fs gl lc1' als Mem cs lc2' als' Mem' tr /\
+    subAL _ lc2 lc2'.
+Proof.
+  intros.
+  destruct db_subEnv as [_ [_ [J _]]].
+  unfold dbSubblocks_subEnv_prop in J. eauto.
+Qed.
+
+Lemma dbBlock_subEnv : forall S TD Ps fs gl F arg tr B1 lc1 als Mem B1' lc2 als' Mem' lc1',
+  dbBlock S TD Ps fs gl F arg 
+    (mkState (mkEC B1 lc1 als) Mem) 
+    (mkState (mkEC B1' lc2 als') Mem') 
+    tr ->
+  subAL _ lc1 lc1' ->
+  exists lc2',
+    dbBlock S TD Ps fs gl F arg 
+     (mkState (mkEC B1 lc1' als) Mem) 
+     (mkState (mkEC B1' lc2' als') Mem') 
+     tr /\
+    subAL _ lc2 lc2'.
+Proof.
+  intros.
+  destruct db_subEnv as [_ [_ [_ [J _]]]].
+  unfold dbBlock_subEnv_prop in J. eauto.
+Qed.
+
+Lemma dbBlocks_subEnv : forall S TD Ps fs gl F lp tr B1 lc1 als Mem B1' lc2 als' Mem' lc1',
+  dbBlocks S TD Ps fs gl F lp
+    (mkState (mkEC B1 lc1 als) Mem)
+    (mkState (mkEC B1' lc2 als') Mem')
+    tr ->
+  subAL _ lc1 lc1' ->
+  exists lc2',
+    dbBlocks S TD Ps fs gl F lp 
+     (mkState (mkEC B1 lc1' als) Mem) 
+     (mkState (mkEC B1' lc2' als') Mem') 
+     tr /\
+    subAL _ lc2 lc2'.
+Proof.
+  intros.
+  destruct db_subEnv as [_ [_ [_ [_ [J _]]]]].
+  unfold dbBlocks_subEnv_prop in J. eauto.
+Qed.
+
+Lemma dbFdef_subEnv : forall fv fid rt lp S TD Ps lc1 gl fs Mem lc2 als' Mem' B' Rid oResult tr la lb lc1',
+  dbFdef fv rt lp S TD Ps lc1 gl fs Mem lc2 als' Mem' B' Rid oResult tr ->
+  lookupFdefViaGV TD Ps gl lc1 fs fv = Some (fdef_intro (fheader_intro rt fid la) lb) ->
+  subAL _ lc1 lc1' ->
+  exists lc2',
+    dbFdef fv rt lp S TD Ps lc1' gl fs Mem lc2' als' Mem' B' Rid oResult tr /\
+    subAL _ lc2 lc2'.
+Proof.
+  intros.
+  destruct db_subEnv as [_ [_ [_ [_ [_ J]]]]].
+  unfold dbFdef_subEnv_prop in J. eauto.
+Qed.
+
+
