src/TV/symexe_tactic.v
@@ -1,0 +1,50 @@
+Add LoadPath "../ssa".
+Require Import Arith.
+Require Import Bool.
+Require Import Coq.Bool.Sumbool.
+Require Import List.
+Require Import ssa_lib.
+Require Import symexe_def.
+Require Import eq_tv.
+Require Import sub_tv.
+
+Export SimpleSE.
+
+Tactic Notation "bdestruct" ident(H) "as" ident(J1) ident(J2) :=
+     apply andb_true_iff in H; destruct H as [J1 J2].
+
+Tactic Notation "bdestruct3" ident(H) "as" ident(J1) ident(J2) ident(J3) :=
+     bdestruct H as H J3;
+     bdestruct H as J1 J2.
+
+Tactic Notation "bdestruct4" ident(H) "as" ident(J1) ident(J2) ident(J3) ident(J4) :=
+     bdestruct3 H as H J3 J4;
+     bdestruct H as J1 J2.
+
+Tactic Notation "bdestruct5" ident(H) "as" ident(J1) ident(J2) ident(J3) ident(J4) ident(J5) :=
+     bdestruct4 H as H J3 J4 J5;
+     bdestruct H as J1 J2.
+
+Ltac bdestructn H Js :=
+  match Js with
+  | nil => idtac
+  | ?J::nil => rename H into J
+  | ?J::?Js' => apply andb_true_iff in H; destruct H as [H J]; bdestructn H Js
+  end.
+
+Ltac sumbool_subst :=
+  repeat
+  match goal with
+  | [ H:sumbool2bool _ _ _ = true |- _ ] => apply sumbool2bool_true in H; subst
+  | [ H:is_true(sumbool2bool _ _ _) |- _ ] => apply sumbool2bool_true in H; subst
+  end.
+
+Tactic Notation "sumbool_subst" "in" hyp(H) :=
+  apply sumbool2bool_true in H.
+
+Ltac bsplit :=
+  eapply andb_true_iff; split.
+
+Ltac repeat_bsplit :=
+  repeat (bsplit; auto using eq_sumbool2bool_true).
+
